fix: 4 admit. rest

algorithms/MaxSum.v
@@ -4,7 +4,6 @@ Require Import Coq.Classes.Morphisms.
 Require Import Coq.Logic.Classical_Prop.
 Require Import Coq.micromega.Psatz.
 Require Import SetsClass.SetsClass.
-Require Import MonadLib.MonadLib.
 From MonadLib.SetMonad Require Import SetBasic SetHoare FixpointLib.
 From MaxMinLib Require Import MaxMin Interface.
 Require Import Algorithms.MapLib.
@@ -29,21 +28,21 @@ Definition max_sum (l: list Z): program (Z * list Z) :=
                            (0, [], 0, []);;
   ret (max1, ans1).
 
-(** Definition of non-adjacent indices:  indices are strictly increasing and no two indices are adjacent *)
+(** Definition of non-adjacent indices: indices are strictly increasing and no two indices are adjacent *)
 Definition non_adjacent_in (il: list Z): Prop :=
-  sincr il /\ forall i j, In i il -> In j il -> i + 1 <> j. 
+  sincr il /\ forall i j, In i il -> In j il -> i + 1 <> j.
 
 (** s is a non-adjacent subsequence of l with index list il *)
-Definition non_adjacent_subseq (s l :  list Z): Prop :=
-  exists il, is_indexed_elements l il s /\ non_adjacent_in il. 
+Definition non_adjacent_subseq (s l : list Z): Prop :=
+  exists il, is_indexed_elements l il s /\ non_adjacent_in il.
 
 (** Definition of sum of a list *)
 Definition sum (l: list Z) : Z := fold_right Z.add 0 l.
 
-(** Definition of the feasible set:  s is feasible if it is a non-adjacent subsequence of l *)
-Definition feasible_set (l :  list Z) (s : list Z) := non_adjacent_subseq s l.
+(** Definition of the feasible set: s is feasible if it is a non-adjacent subsequence of l *)
+Definition feasible_set (l : list Z) (s : list Z) := non_adjacent_subseq s l.
 
-(** Specification for the maximum value:  m is the maximum sum among all feasible subsequences *)
+(** Specification for the maximum value: m is the maximum sum among all feasible subsequences *)
 Definition max_value_spec (l: list Z) (m: Z) : Prop :=
   (exists s,
       feasible_set l s /\
@@ -56,23 +55,23 @@ Definition max_value_spec (l: list Z) (m: Z) : Prop :=
 Definition max_sum_full_spec (l: list Z) (m: Z) (s: list Z) : Prop :=
   max_value_spec l m /\
   feasible_set l s /\
-  sum s = m. 
+  sum s = m.
 
-Lemma sum_app:  forall l1 l2, sum (l1 ++ l2) = sum l1 + sum l2.
-Proof. 
+Lemma sum_app: forall l1 l2, sum (l1 ++ l2) = sum l1 + sum l2.
+Proof.
   intros. induction l1; simpl; auto.
-  rewrite IHl1. apply Z.add_assoc. 
+  rewrite IHl1. apply Z.add_assoc.
 Qed.
 
 Lemma feasible_set_nil: forall s, feasible_set [] s -> s = [].
-Proof.  
-  intros s H. 
+Proof. 
+  intros s H.
   unfold feasible_set, non_adjacent_subseq in H.  
   destruct H as [il [Hidx _]].  
   destruct s as [| a s'].
-  - reflexivity.  
+  - reflexivity. 
   - exfalso. 
-    apply is_indexed_elements_cons_inv_r in Hidx.  
+    apply is_indexed_elements_cons_inv_r in Hidx. 
     destruct Hidx as [i [il' [_ [Hnth _]]]].
     unfold Znth_error in Hnth.
     destruct (Z_le_gt_dec 0 i).
@@ -80,36 +79,36 @@ Proof.
       assert (nth_error (@nil Z) (Z.to_nat i) = None) by (destruct (Z.to_nat i); reflexivity).
       congruence.
     + 
-      discriminate Hnth.   
-Qed. 
+      discriminate Hnth. 
+Qed.
 
 Lemma feasible_set_nil_intro: feasible_set [] [].
 Proof.
   exists []. split.
-  - apply is_indexed_elements_nil. 
+  - apply is_indexed_elements_nil.
   - split; simpl; auto.
 Qed.
 
 Lemma max_value_spec_nil: max_value_spec [] 0.
 Proof.
-  left. exists []. split; [| split]. 
-  - apply feasible_set_nil_intro. 
+  left. exists []. split; [| split].
+  - apply feasible_set_nil_intro.
   - reflexivity.
-  - intros t H.  apply feasible_set_nil in H.  subst.  simpl.  lia.
-Qed. 
+  - intros t H. apply feasible_set_nil in H. subst. simpl. lia.
+Qed.
 
 Lemma Znth_error_app_l: forall {A} (l1 l2: list A) i,
   0 <= i < Zlength l1 ->
-  Znth_error (l1 ++ l2) i = Znth_error l1 i. 
+  Znth_error (l1 ++ l2) i = Znth_error l1 i.
 Proof.
-  intros. 
-  unfold Znth_error. 
-  destruct H as [Hge Hlt].  
+  intros.
+  unfold Znth_error.
+  destruct H as [Hge Hlt]. 
   destruct (Z_le_gt_dec 0 i); try lia.
-  rewrite nth_error_app1. 
+  rewrite nth_error_app1.
   - reflexivity.
-  - unfold Zlength in Hlt. 
-    apply Z2Nat.inj_lt in Hlt; try lia. 
+  - unfold Zlength in Hlt.
+    apply Z2Nat.inj_lt in Hlt; try lia.
 Qed.
 
 Lemma Znth_error_app_r: forall {A} (l1 l2: list A) i,
@@ -122,18 +121,18 @@ Proof.
   - 
     destruct (Z_le_gt_dec 0 (i - Zlength l1)).
     + 
-      rewrite nth_error_app2. 
+      rewrite nth_error_app2.
       * f_equal.
         rewrite Z2Nat.inj_sub; try lia.
-        -- unfold Zlength.  rewrite Nat2Z.id. reflexivity.
+        -- unfold Zlength. rewrite Nat2Z.id. reflexivity.
         -- unfold Zlength. lia.
-      * unfold Zlength in H. apply Z2Nat.inj_le in H; try lia. 
+      * unfold Zlength in H. apply Z2Nat.inj_le in H; try lia.
     +
       lia.
   - 
     pose proof (Zlength_nonneg l1).
     lia.
-Qed. 
+Qed.
 
 Lemma feasible_set_app_x_l: forall l x s,
   feasible_set l s -> feasible_set (l ++ [x]) s.
@@ -141,12 +140,13 @@ Proof.
   intros l x s [il [Hidx [Hsincr Hgap]]].
   exists il. split; [| split; auto].
   - apply is_indexed_elements_range in Hidx as Hrange.
-    eapply Forall2_congr; [| eauto]. 
+    eapply Forall2_congr; [| eauto].
     intros i a Hin1 Hin2 Hnth.
     rewrite Forall_forall in Hrange.
     specialize (Hrange _ Hin1).
-    rewrite Znth_error_app_l; auto. 
+    rewrite Znth_error_app_l; auto.
 Qed.
+
 
 Lemma Znth_error_snoc_last: forall {A} (l: list A) x,
   Znth_error (l ++ [x]) (Zlength l) = Some x.
@@ -155,61 +155,62 @@ Proof.
   rewrite Znth_error_app_r; [| lia].
   replace (Zlength l - Zlength l) with 0 by lia.
   apply Znth_error_cons_0.
-Qed. 
+Qed.
 
 Lemma is_indexed_elements_extend: forall (l: list Z) x s (il: list Z),
   is_indexed_elements (removelast l) il s ->
   is_indexed_elements (l ++ [x]) il s.
 Proof.
-  intros. 
-  destruct l. 
-  - 
+  intros.
+  destruct l.
+  - (* Case l = [] *)
     simpl in H.
     unfold is_indexed_elements in *.
-    destruct il. 
-    + inversion H; subst.  apply Forall2_nil.
-    + inversion H; subst. 
+    destruct il.
+    + inversion H; subst. apply Forall2_nil.
+    + inversion H; subst.
       unfold Znth_error in H2.
       destruct (Z_le_gt_dec 0 z).
-      * destruct (Z.to_nat z); simpl in H2; discriminate. 
-      * discriminate. 
+      * destruct (Z.to_nat z); simpl in H2; discriminate.
+      * discriminate.
   - 
     unfold is_indexed_elements in *.
-    eapply Forall2_congr; [| eauto]. 
+    eapply Forall2_congr; [| eauto].
     intros i a0 Hin_i Hin_s Hnth.
-    assert (Hneq: z ::  l <> []) by congruence.
+    assert (Hneq: z :: l <> []) by congruence.
     destruct (exists_last Hneq) as [l' [a Heq]].
     rewrite Heq in Hnth.
-    rewrite Heq. 
+    rewrite Heq.
     
     rewrite removelast_app in Hnth; [| discriminate].
-    simpl in Hnth. 
-    rewrite app_nil_r in Hnth. 
-    rewrite <- app_assoc. 
+    simpl in Hnth.
+    rewrite app_nil_r in Hnth.
+    rewrite <- app_assoc.
     rewrite Znth_error_app_l.
     + 
       assumption.
     + 
       apply Znth_error_range in Hnth.
       assumption.
-Qed. 
+Qed.
 
-Lemma is_indexed_elements_prefix_extend : 
-  forall (l :  list Z) (x : Z) (s il :  list Z),
+Lemma is_indexed_elements_prefix_extend :
+  forall (l : list Z) (x : Z) (s il : list Z),
     is_indexed_elements l il s ->
     is_indexed_elements (l ++ [x]) il s.
 Proof.
-  intros l x s il H. 
+  intros l x s il H.
   unfold is_indexed_elements in *.
-  induction H as [| i a il' s' Hnth Hrest IH]; simpl. 
-  - apply Forall2_nil. 
-  - apply Forall2_cons. 
+  induction H as [| i a il' s' Hnth Hrest IH]; simpl.
+  - apply Forall2_nil.
+  - apply Forall2_cons.
     + assert (Hrange: 0 <= i < Zlength l).
-      { apply Znth_error_range in Hnth.  tauto. }
+      { apply Znth_error_range in Hnth. tauto. }
       rewrite (Znth_error_app_l _ _ _ Hrange).
       exact Hnth.
-    + apply IH. 
+    + apply IH.
 Qed.
+
 
 Lemma sincr_extend_last: forall (il: list Z) (last_idx: Z),
   sincr il ->
@@ -217,9 +218,9 @@ Lemma sincr_extend_last: forall (il: list Z) (last_idx: Z),
   sincr (il ++ [last_idx]).
 Proof.
   intros il last_idx Hsincr Hlast.
-  destruct il as [| i0 il'].  
+  destruct il as [| i0 il']. 
   - 
-    simpl.   auto.
+    simpl.  auto.
   - 
     simpl in *.
     destruct Hlast as [Heq | Hlt].
@@ -234,10 +235,10 @@ Proof.
         split; auto.
       * 
         simpl in Hsincr.
-        destruct Hsincr as [Hi0_i1 Hrest].  
-        simpl.  
+        destruct Hsincr as [Hi0_i1 Hrest]. 
+        simpl. 
         split; [exact Hi0_i1 | ].
-        apply IH; auto. 
+        apply IH; auto.
 Qed.
 
 Lemma sincr_app_singleton_inv: forall l1 x,
@@ -246,134 +247,134 @@ Lemma sincr_app_singleton_inv: forall l1 x,
 Proof.
   induction l1 as [| a l1' IH]; intros x Hsincr i Hin.
   - inversion Hin.
-  - simpl in Hsincr. 
-    simpl in Hin.  
+  - simpl in Hsincr.
+    simpl in Hin. 
     destruct Hin as [Heq | Hin']. 
     + subst i.
       destruct l1' as [| b l1''].
       * 
-        simpl in Hsincr.  
+        simpl in Hsincr. 
         lia.
       * 
-        simpl in Hsincr.  
-        destruct Hsincr as [Hab Hrest]. 
+        simpl in Hsincr. 
+        destruct Hsincr as [Hab Hrest].
         assert (Hbx: b < x).
         { apply (IH x); auto. left; reflexivity. }
         lia.
     + apply IH; auto.
       destruct l1' as [| b l1'']; simpl in *; tauto.
-Qed.  
+Qed. 
 
-Lemma last_in_list:   forall {A} (l:   list A) (d: A),
+Lemma last_in_list:  forall {A} (l:  list A) (d: A),
   l <> [] -> In (last l d) l.
 Proof.
   intros A l d Hneq.
-  induction l as [| a l' IH]. 
-  - contradiction. 
+  induction l as [| a l' IH].
+  - contradiction.
   - destruct l' as [| b l'']. 
-    + simpl.   left.  reflexivity.
-    + simpl.  right. apply IH.  discriminate.
-Qed.  
+    + simpl.  left. reflexivity.
+    + simpl. right. apply IH.  discriminate.
+Qed. 
 
-Lemma feasible_set_app_x_r:   forall l x s,
+Lemma feasible_set_app_x_r:  forall l x s,
   feasible_set (removelast l) s -> feasible_set (l ++ [x]) (s ++ [x]).
 Proof.
   intros l x s H.
   unfold feasible_set, non_adjacent_subseq in *.
   destruct H as [il [Hidx [Hsincr Hgap]]].  
   exists (il ++ [Zlength l]).
-  split; [| split].  
+  split; [| split]. 
   
   - 
-    apply is_indexed_elements_app.  
+    apply is_indexed_elements_app. 
     + 
-      apply is_indexed_elements_extend.  
+      apply is_indexed_elements_extend. 
       exact Hidx. 
     + 
-      apply is_indexed_elements_cons. 
+      apply is_indexed_elements_cons.
       * 
         apply Znth_error_snoc_last.
       *
-        apply is_indexed_elements_nil.  
+        apply is_indexed_elements_nil. 
   
   - 
-    apply sincr_extend_last.  
+    apply sincr_extend_last. 
     + exact Hsincr.
     + destruct il as [| i0 il']. 
-      * left. reflexivity.  
+      * left. reflexivity. 
       * right. 
-        apply is_indexed_elements_range in Hidx.  
-        rewrite Forall_forall in Hidx. 
+        apply is_indexed_elements_range in Hidx. 
+        rewrite Forall_forall in Hidx.
         assert (Hin_last: In (last (i0 :: il') 0) (i0 :: il')).
-        { apply last_in_list.   discriminate. }
+        { apply last_in_list.  discriminate. }
         specialize (Hidx _ Hin_last).
-        destruct (list_snoc_destruct l) as [Heq_l | [a [l0 Heq_l]]]. 
+        destruct (list_snoc_destruct l) as [Heq_l | [a [l0 Heq_l]]].
         -- 
-           subst l.   simpl in Hidx.   unfold Zlength in *. simpl in *. lia.
+           subst l.  simpl in Hidx.  unfold Zlength in *. simpl in *. lia.
         -- 
-           subst l.  
+           subst l. 
            rewrite removelast_app in Hidx by discriminate.
-           simpl in Hidx.  rewrite app_nil_r in Hidx.  
-           rewrite Zlength_app.   unfold Zlength in *. simpl in *.  lia.
+           simpl in Hidx. rewrite app_nil_r in Hidx. 
+           rewrite Zlength_app.  unfold Zlength in *. simpl in *.  lia.
   
   - 
     intros i j Hi Hj.
-    apply in_app_or in Hi.  
+    apply in_app_or in Hi. 
     apply in_app_or in Hj.
     destruct Hi as [Hi_il | Hi_last];
-    destruct Hj as [Hj_il | Hj_last].    
+    destruct Hj as [Hj_il | Hj_last].   
     + 
       apply Hgap; auto.
     + 
-      simpl in Hj_last.  
-      destruct Hj_last as [Heq | Hf]; [| contradiction].  
-      subst j. 
+      simpl in Hj_last. 
+      destruct Hj_last as [Heq | Hf]; [| contradiction]. 
+      subst j.
       apply is_indexed_elements_range in Hidx.
       rewrite Forall_forall in Hidx.
       specialize (Hidx _ Hi_il).
-      destruct (list_snoc_destruct l) as [Heq_l | [a [l0 Heq_l]]].  
-      * subst l.   simpl in Hidx.  unfold Zlength in *.  simpl in *. lia.   
-      * subst l.  
-        rewrite removelast_app in Hidx by discriminate.   
-        simpl in Hidx.    rewrite app_nil_r in Hidx. 
-        rewrite Zlength_app.  unfold Zlength in *.  simpl in *. 
+      destruct (list_snoc_destruct l) as [Heq_l | [a [l0 Heq_l]]]. 
+      * subst l.  simpl in Hidx. unfold Zlength in *. simpl in *. lia.  
+      * subst l. 
+        rewrite removelast_app in Hidx by discriminate.  
+        simpl in Hidx.   rewrite app_nil_r in Hidx.
+        rewrite Zlength_app. unfold Zlength in *. simpl in *.
         lia.  
     + 
-      simpl in Hi_last. 
-      destruct Hi_last as [Heq | Hf]; [| contradiction].   
-      subst i.  
-      apply is_indexed_elements_range in Hidx.  
-      rewrite Forall_forall in Hidx. 
+      simpl in Hi_last.
+      destruct Hi_last as [Heq | Hf]; [| contradiction].  
+      subst i. 
+      apply is_indexed_elements_range in Hidx. 
+      rewrite Forall_forall in Hidx.
       specialize (Hidx _ Hj_il).
-      destruct (list_snoc_destruct l) as [Heq_l | [a [l0 Heq_l]]].   
-      * subst l.  simpl in Hidx. unfold Zlength in *. simpl in *.  lia. 
-      * subst l. 
-        rewrite removelast_app in Hidx by discriminate. 
-        simpl in Hidx.  rewrite app_nil_r in Hidx.  
+      destruct (list_snoc_destruct l) as [Heq_l | [a [l0 Heq_l]]].  
+      * subst l.  simpl in Hidx. unfold Zlength in *. simpl in *.  lia.
+      * subst l.
+        rewrite removelast_app in Hidx by discriminate.
+        simpl in Hidx. rewrite app_nil_r in Hidx. 
         rewrite Zlength_app. unfold Zlength in *. simpl in *. 
-        lia.  
+        lia. 
     + 
       simpl in Hi_last, Hj_last.
-      destruct Hi_last as [Heq_i | Hf]; [| contradiction]. 
+      destruct Hi_last as [Heq_i | Hf]; [| contradiction].
       destruct Hj_last as [Heq_j | Hf]; [| contradiction].
       subst i j.
-      lia.  
-Qed.  
+      lia. 
+Qed. 
 
-Lemma feasible_set_app_x_inv_empty_il:  forall l x s,
+Lemma feasible_set_app_x_inv_empty_il: forall l x s,
   is_indexed_elements (l ++ [x]) [] s ->
-  feasible_set l s.  
+  feasible_set l s. 
 Proof.
   intros l x s Hidx.
   apply is_indexed_elements_nil_inv_l in Hidx. 
   subst s.
-  exists []. 
-  split.  
+  exists [].
+  split. 
   - apply is_indexed_elements_nil.
-  - split; simpl; auto. 
-Qed.  
+  - split; simpl; auto.
+Qed. 
 
-Lemma feasible_set_app_x_inv_l_empty:    forall (x:    Z) il' s1,
+Lemma feasible_set_app_x_inv_l_empty:   forall (x:   Z) il' s1,
   sincr (il' ++ [0]) ->
   is_indexed_elements ([] ++ [x]) il' s1 ->
   il' = [] /\ s1 = [].  
@@ -381,43 +382,43 @@ Proof.
   intros x il' s1 Hsincr Hidx1.
   simpl in Hidx1.
   destruct il' as [| i0 il''].   
-  - split; auto. 
-    apply is_indexed_elements_nil_inv_l in Hidx1.  auto. 
-  - exfalso.   
+  - split; auto.
+    apply is_indexed_elements_nil_inv_l in Hidx1.  auto.
+  - exfalso.  
     apply is_indexed_elements_cons_inv_l in Hidx1.
     destruct Hidx1 as [a1 [s1' [Hnth0 _]]].  
     unfold Znth_error in Hnth0.
     destruct (Z_le_gt_dec 0 i0).
     + simpl in Hsincr.   
       destruct il'' as [| i1 il'''].  
-      * simpl in Hsincr.  
+      * simpl in Hsincr. 
         destruct Hsincr as [Hi0_lt_0 _].   
         lia.
-      * simpl in Hsincr.  
+      * simpl in Hsincr. 
         destruct Hsincr as [Hi0_lt_i1 Hrest].  
         assert (Hi1_lt_0: i1 < 0).
         {
-          clear -Hrest.  
+          clear -Hrest. 
           assert (Haux: forall il y,
                      sincr_aux il y ->
                      forall j, In j il -> y < j).
           {
-            clear.   
-            induction il as [| a il' IH]; intros y Hsaux j Hin. 
-            - inversion Hin.  
-            - simpl in Hsaux. destruct Hsaux as [Hya Hrest'].     
-              simpl in Hin.   destruct Hin as [Heq | Hin'].  
-              + subst.   exact Hya.  
-              + assert (Ha_lt_j:    a < j) by (apply IH; auto). lia.
+            clear.  
+            induction il as [| a il' IH]; intros y Hsaux j Hin.
+            - inversion Hin. 
+            - simpl in Hsaux. destruct Hsaux as [Hya Hrest'].    
+              simpl in Hin.  destruct Hin as [Heq | Hin'].  
+              + subst.  exact Hya. 
+              + assert (Ha_lt_j:   a < j) by (apply IH; auto). lia.
           }
           apply (Haux (il''' ++ [0]) i1 Hrest 0).
-          apply in_app_iff.     right.   simpl. left.   reflexivity. 
+          apply in_app_iff.    right.  simpl. left.  reflexivity. 
         }
-        lia.  
+        lia. 
     + discriminate Hnth0.
-Qed.  
+Qed. 
 
-Lemma feasible_set_app_x_inv_idx_bound: forall (l0 :    list Z) (a0 x :  Z) il' i,
+Lemma feasible_set_app_x_inv_idx_bound: forall (l0 :   list Z) (a0 x : Z) il' i,
   sincr (il' ++ [Zlength (l0 ++ [a0])]) ->
   (forall i j, In i (il' ++ [Zlength (l0 ++ [a0])]) -> 
                In j (il' ++ [Zlength (l0 ++ [a0])]) -> 
@@ -426,43 +427,43 @@ Lemma feasible_set_app_x_inv_idx_bound: forall (l0 :    list Z) (a0 x :  Z) il' 
   (exists s1, is_indexed_elements ((l0 ++ [a0]) ++ [x]) il' s1) ->
   (exists a, Znth_error ((l0 ++ [a0]) ++ [x]) i = Some a) ->
   i < Zlength l0.
-Proof.  
+Proof. 
   intros l0 a0 x il' i Hsincr Hgap Hin_i [s1 Hidx] _. 
-  assert (Hi_lt:   i < Zlength (l0 ++ [a0])).
+  assert (Hi_lt:  i < Zlength (l0 ++ [a0])).
   { apply sincr_app_singleton_inv with (l1 := il'); auto. }
   apply is_indexed_elements_range in Hidx.
   rewrite Forall_forall in Hidx.
-  specialize (Hidx i Hin_i) as [Hi_ge _]. 
+  specialize (Hidx i Hin_i) as [Hi_ge _].
   assert (Hneq: i + 1 <> Zlength (l0 ++ [a0])).
   {
     apply Hgap.
-    - apply in_app_iff.  left. exact Hin_i.
-    - apply in_app_iff.  right. simpl. left.   reflexivity.  
+    - apply in_app_iff. left. exact Hin_i.
+    - apply in_app_iff. right. simpl. left.  reflexivity. 
   }
   unfold Zlength in *.
-  rewrite length_app in Hi_lt, Hneq.  
-  simpl in Hi_lt, Hneq.  
-  lia. 
-Qed.  
+  rewrite length_app in Hi_lt, Hneq. 
+  simpl in Hi_lt, Hneq. 
+  lia.
+Qed. 
 
-Lemma sincr_app_cons_inv1:   forall l1 x,
+Lemma sincr_app_cons_inv1:  forall l1 x,
   sincr (l1 ++ [x]) ->
   sincr l1.
 Proof.
   intros l1 x Hsincr.
-  destruct l1 as [| a l1'].  
-  - simpl.   auto.
-  - simpl in Hsincr |- *. 
-    revert a Hsincr. 
-    induction l1' as [| b l1'' IH]; intros a Hsincr.  
-    + simpl in *. auto. 
+  destruct l1 as [| a l1']. 
+  - simpl.  auto.
+  - simpl in Hsincr |- *.
+    revert a Hsincr.
+    induction l1' as [| b l1'' IH]; intros a Hsincr. 
+    + simpl in *. auto.
     + simpl in Hsincr |- *.
       destruct Hsincr as [Hab Hrest].
       split; [exact Hab |].
-      apply IH.   exact Hrest.
+      apply IH.  exact Hrest.
 Qed. 
 
-Lemma feasible_set_app_x_inv_i_last_eq:   forall l x s il' i_last,
+Lemma feasible_set_app_x_inv_i_last_eq:  forall l x s il' i_last,
   i_last = Zlength l ->
   sincr (il' ++ [i_last]) ->
   (forall i j, In i (il' ++ [i_last]) -> In j (il' ++ [i_last]) -> i + 1 <> j) ->
@@ -470,117 +471,117 @@ Lemma feasible_set_app_x_inv_i_last_eq:   forall l x s il' i_last,
   exists s', s = s' ++ [x] /\ feasible_set (removelast l) s'.
 Proof.
   intros l x s il' i_last Heq_idx Hsincr Hgap Hidx.
-  apply is_indexed_elements_app_inv_l in Hidx. 
-  destruct Hidx as [s1 [s2 [Hidx1 [Hidx2 Heq_s]]]].   
-  subst s.  
-  apply is_indexed_elements_cons_inv_l in Hidx2.
-  destruct Hidx2 as [a [s2' [Hnth_last [Hidx2' Heq_s2]]]].  
-  apply is_indexed_elements_nil_inv_l in Hidx2'.   
-  subst s2 s2'.  
-  rewrite Heq_idx in Hnth_last.  
-  rewrite Znth_error_snoc_last in Hnth_last.  
-  injection Hnth_last as Heq_a.  
-  subst a. 
-  exists s1. 
-  split; [reflexivity |].  
-  unfold feasible_set, non_adjacent_subseq.    
-  exists il'. 
-  split; [| split].  
-  -
-    destruct (list_snoc_destruct l) as [Heq_l | [a0 [l0 Heq_l]]].  
-    + 
-      subst l. 
-      simpl in Heq_idx.  
-      unfold Zlength in Heq_idx.  
-      simpl in Heq_idx.   
-      subst i_last.  
-      apply feasible_set_app_x_inv_l_empty in Hidx1 as [Hil' Hs1]; auto.  
-      subst il' s1.
-      simpl.  
-      apply is_indexed_elements_nil.   
-    + 
-      subst l. 
-      rewrite removelast_app by discriminate.  
-      simpl.   rewrite app_nil_r.  
-      assert (Hidx1_saved:   is_indexed_elements ((l0 ++ [a0]) ++ [x]) il' s1) by exact Hidx1.
-      eapply Forall2_congr; [| exact Hidx1].    
-      intros i a Hin_i Hin_s Hnth.  
-      assert (Hlt:   i < Zlength l0).
-      {
-        eapply feasible_set_app_x_inv_idx_bound with (a0 := a0) (x := x) (il' := il').
-        - 
-          assert (Heq_i_last: i_last = Zlength (l0 ++ [a0])).
-          { rewrite <- Heq_idx.   reflexivity.   }
-          rewrite <- Heq_i_last. 
-          exact Hsincr.
-        - 
-          intros i' j' Hi' Hj'.  
-          assert (Heq_i_last:    i_last = Zlength (l0 ++ [a0])).
-          { rewrite <- Heq_idx.  reflexivity. }
-          rewrite <- Heq_i_last in Hi', Hj'.
-          apply Hgap; auto.  
-        - exact Hin_i.  
-        - exists s1. exact Hidx1_saved.  
-        - exists a.    exact Hnth.  
-      }
-      symmetry. 
-      assert (Hnth_range:   0 <= i < Zlength ((l0 ++ [a0]) ++ [x])).
-      { apply Znth_error_range in Hnth.   exact Hnth. }
-      replace ((l0 ++ [a0]) ++ [x]) with (l0 ++ ([a0] ++ [x])) in Hnth by (rewrite app_assoc; reflexivity).
-      rewrite Znth_error_app_l in Hnth.  
-      * symmetry.  exact Hnth. 
-      * split.  
-        -- destruct Hnth_range.  lia.
-        -- exact Hlt. 
-  - 
-    apply sincr_app_cons_inv1 with (x := i_last).
-    exact Hsincr.
-  - 
-    intros i j Hi Hj.  
-    apply Hgap. 
-    + apply in_app_iff.    left.  exact Hi.  
-    + apply in_app_iff.  left.  exact Hj. 
-Qed.  
-
-Lemma feasible_set_app_x_inv_i_last_neq:  forall l x s il' i_last,
-  i_last <> Zlength l ->
-  sincr (il' ++ [i_last]) ->
-  (forall i j, In i (il' ++ [i_last]) -> In j (il' ++ [i_last]) -> i + 1 <> j) ->
-  is_indexed_elements (l ++ [x]) (il' ++ [i_last]) s ->
-  feasible_set l s. 
-Proof.
-  intros l x s il' i_last Hneq Hsincr Hgap Hidx.  
   apply is_indexed_elements_app_inv_l in Hidx.
-  destruct Hidx as [s1 [s2 [Hidx1 [Hidx2 Heq_s]]]]. 
+  destruct Hidx as [s1 [s2 [Hidx1 [Hidx2 Heq_s]]]].   
   subst s. 
   apply is_indexed_elements_cons_inv_l in Hidx2.
   destruct Hidx2 as [a [s2' [Hnth_last [Hidx2' Heq_s2]]]]. 
   apply is_indexed_elements_nil_inv_l in Hidx2'.  
   subst s2 s2'. 
+  rewrite Heq_idx in Hnth_last. 
+  rewrite Znth_error_snoc_last in Hnth_last.  
+  injection Hnth_last as Heq_a. 
+  subst a. 
+  exists s1.
+  split; [reflexivity |].  
+  unfold feasible_set, non_adjacent_subseq.   
+  exists il'. 
+  split; [| split]. 
+  -
+    destruct (list_snoc_destruct l) as [Heq_l | [a0 [l0 Heq_l]]].  
+    + 
+      subst l.
+      simpl in Heq_idx. 
+      unfold Zlength in Heq_idx.  
+      simpl in Heq_idx.  
+      subst i_last. 
+      apply feasible_set_app_x_inv_l_empty in Hidx1 as [Hil' Hs1]; auto. 
+      subst il' s1.
+      simpl. 
+      apply is_indexed_elements_nil.  
+    + 
+      subst l.
+      rewrite removelast_app by discriminate. 
+      simpl.  rewrite app_nil_r. 
+      assert (Hidx1_saved:  is_indexed_elements ((l0 ++ [a0]) ++ [x]) il' s1) by exact Hidx1.
+      eapply Forall2_congr; [| exact Hidx1].   
+      intros i a Hin_i Hin_s Hnth. 
+      assert (Hlt:  i < Zlength l0).
+      {
+        eapply feasible_set_app_x_inv_idx_bound with (a0 := a0) (x := x) (il' := il').
+        - 
+          assert (Heq_i_last: i_last = Zlength (l0 ++ [a0])).
+          { rewrite <- Heq_idx.  reflexivity.  }
+          rewrite <- Heq_i_last.
+          exact Hsincr.
+        - 
+          intros i' j' Hi' Hj'.  
+          assert (Heq_i_last:   i_last = Zlength (l0 ++ [a0])).
+          { rewrite <- Heq_idx. reflexivity. }
+          rewrite <- Heq_i_last in Hi', Hj'.
+          apply Hgap; auto.  
+        - exact Hin_i.  
+        - exists s1. exact Hidx1_saved.  
+        - exists a.   exact Hnth. 
+      }
+      symmetry. 
+      assert (Hnth_range:  0 <= i < Zlength ((l0 ++ [a0]) ++ [x])).
+      { apply Znth_error_range in Hnth.  exact Hnth. }
+      replace ((l0 ++ [a0]) ++ [x]) with (l0 ++ ([a0] ++ [x])) in Hnth by (rewrite app_assoc; reflexivity).
+      rewrite Znth_error_app_l in Hnth. 
+      * symmetry.  exact Hnth.
+      * split. 
+        -- destruct Hnth_range.  lia.
+        -- exact Hlt.
+  - 
+    apply sincr_app_cons_inv1 with (x := i_last).
+    exact Hsincr.
+  - 
+    intros i j Hi Hj. 
+    apply Hgap. 
+    + apply in_app_iff.   left.  exact Hi. 
+    + apply in_app_iff. left.  exact Hj. 
+Qed.  
+
+Lemma feasible_set_app_x_inv_i_last_neq: forall l x s il' i_last,
+  i_last <> Zlength l ->
+  sincr (il' ++ [i_last]) ->
+  (forall i j, In i (il' ++ [i_last]) -> In j (il' ++ [i_last]) -> i + 1 <> j) ->
+  is_indexed_elements (l ++ [x]) (il' ++ [i_last]) s ->
+  feasible_set l s.
+Proof.
+  intros l x s il' i_last Hneq Hsincr Hgap Hidx. 
+  apply is_indexed_elements_app_inv_l in Hidx.
+  destruct Hidx as [s1 [s2 [Hidx1 [Hidx2 Heq_s]]]].
+  subst s. 
+  apply is_indexed_elements_cons_inv_l in Hidx2.
+  destruct Hidx2 as [a [s2' [Hnth_last [Hidx2' Heq_s2]]]].
+  apply is_indexed_elements_nil_inv_l in Hidx2'. 
+  subst s2 s2'.
   assert (Hi_last_range:  0 <= i_last < Zlength (l ++ [x])).
-  { apply Znth_error_range in Hnth_last.  exact Hnth_last.  }
+  { apply Znth_error_range in Hnth_last. exact Hnth_last. }
   assert (Hi_last_lt: i_last < Zlength l).
   {
-    destruct Hi_last_range as [_ Hi_ub]. 
-    rewrite Zlength_app in Hi_ub. 
+    destruct Hi_last_range as [_ Hi_ub].
+    rewrite Zlength_app in Hi_ub.
     unfold Zlength in Hi_ub at 2.
     simpl in Hi_ub. 
-    lia. 
+    lia.
   }
-  assert (Hnth_last_l:  Znth_error l i_last = Some a).
+  assert (Hnth_last_l: Znth_error l i_last = Some a).
   {
-    assert (Hnth_last_copy: Znth_error (l ++ [x]) i_last = Some a) by exact Hnth_last.  
-    rewrite Znth_error_app_l in Hnth_last_copy.  
-    - exact Hnth_last_copy. 
-    - split.  
-      + apply Znth_error_range in Hnth_last.   lia.
+    assert (Hnth_last_copy: Znth_error (l ++ [x]) i_last = Some a) by exact Hnth_last. 
+    rewrite Znth_error_app_l in Hnth_last_copy. 
+    - exact Hnth_last_copy.
+    - split. 
+      + apply Znth_error_range in Hnth_last.  lia.
       + exact Hi_last_lt.
   }
-  unfold feasible_set, non_adjacent_subseq.  
+  unfold feasible_set, non_adjacent_subseq. 
   exists (il' ++ [i_last]).
-  split; [| split]. 
+  split; [| split].
   - 
-    apply is_indexed_elements_app.  
+    apply is_indexed_elements_app. 
     + 
       eapply Forall2_congr; [| exact Hidx1].
       intros i a' Hin_i Hin_s Hnth.  
@@ -589,43 +590,47 @@ Proof.
       { apply sincr_app_singleton_inv with (l1 := il'); auto. }
       assert (Hnth_l: Znth_error l i = Some a').
       {
-        assert (Hnth_copy: Znth_error (l ++ [x]) i = Some a') by exact Hnth.  
+        assert (Hnth_copy: Znth_error (l ++ [x]) i = Some a') by exact Hnth. 
         rewrite Znth_error_app_l in Hnth_copy.
         - exact Hnth_copy. 
-        - split. 
+        - split.
           + apply Znth_error_range in Hnth.  lia.
           + lia.
       }
-      symmetry. exact Hnth_l. 
+      symmetry. exact Hnth_l.
     + 
-      apply is_indexed_elements_cons.  
-      * exact Hnth_last_l. 
-      * apply is_indexed_elements_nil.  
+      apply is_indexed_elements_cons. 
+      * exact Hnth_last_l.
+      * apply is_indexed_elements_nil. 
   - 
     exact Hsincr.
   - 
-    exact Hgap.  
-Qed. 
+    exact Hgap. 
+Qed.
 
-Lemma feasible_set_app_x_inv:   forall l x s,
+Lemma feasible_set_app_x_inv:  forall l x s,
   feasible_set (l ++ [x]) s ->
   feasible_set l s \/
   (exists s', s = s' ++ [x] /\ feasible_set (removelast l) s').
 Proof.
-  intros l x s H. 
+  intros l x s H.
   unfold feasible_set, non_adjacent_subseq in H.
   destruct H as [il [Hidx [Hsincr Hgap]]].   
   destruct (list_snoc_destruct il) as [Heq_il | [i_last [il' Heq_il]]]; subst il.
-  - left.  
+  - 
+    left.
     apply (feasible_set_app_x_inv_empty_il l x s); auto.
-  - destruct (Z.eq_dec i_last (Zlength l)) as [Heq_idx | Hneq_idx].  
-    * right.
-      apply (feasible_set_app_x_inv_i_last_eq l x s il' i_last Heq_idx Hsincr Hgap Hidx).
-    * left.  
-      apply (feasible_set_app_x_inv_i_last_neq l x s il' i_last Hneq_idx Hsincr Hgap Hidx).
+  -
+    destruct (Z.eq_dec i_last (Zlength l)) as [Heq_idx | Hneq_idx]. 
+    + 
+      right.
+      eapply (feasible_set_app_x_inv_i_last_eq l x s il' i_last); eassumption.
+    + 
+      left.
+      eapply (feasible_set_app_x_inv_i_last_neq l x s il' i_last); eassumption. 
 Qed.
 
-Lemma max_value_spec_app: 
+Lemma max_value_spec_app:
   forall l x m1 m2,
     max_value_spec l m1 ->
     max_value_spec (removelast l) m2 ->
@@ -635,28 +640,28 @@ Proof.
   assert (H1: (exists s, feasible_set l s /\ sum s = m1) /\ (forall t, feasible_set l t -> sum t <= m1)).
   {
     destruct Hspec1 as [Hcase1 | Hcase2].
-    - destruct Hcase1 as [s [?  [?  ? ]]]. split; [exists s; auto | auto].
-    - destruct Hcase2 as [Hle Heq].  split; [| subst; auto]. 
-      exists [].  split. 
-      + exists []. split.  apply is_indexed_elements_nil.  split; [simpl; auto | intros; contradiction].
+    - destruct Hcase1 as [s [? [? ?]]]. split; [exists s; auto | auto].
+    - destruct Hcase2 as [Hle Heq]. split; [| subst; auto].
+      exists []. split.
+      + exists []. split. apply is_indexed_elements_nil. split; [simpl; auto | intros; contradiction].
       + subst. reflexivity.
   }
-  destruct H1 as [[s1 [Hfeas1 Hsum1]] Hmax1]. 
+  destruct H1 as [[s1 [Hfeas1 Hsum1]] Hmax1].
 
   assert (H2: (exists s, feasible_set (removelast l) s /\ sum s = m2) /\ (forall t, feasible_set (removelast l) t -> sum t <= m2)).
   {
-    destruct Hspec2 as [Hcase1 | Hcase2]. 
-    - destruct Hcase1 as [s [? [?  ?]]]. split; [exists s; auto | auto].
-    - destruct Hcase2 as [Hle Heq].  split; [| subst; auto].
-      exists []. split. 
-      + exists []. split.  apply is_indexed_elements_nil. split; [simpl; auto | intros; contradiction].
-      + subst. reflexivity. 
+    destruct Hspec2 as [Hcase1 | Hcase2].
+    - destruct Hcase1 as [s [? [? ?]]]. split; [exists s; auto | auto].
+    - destruct Hcase2 as [Hle Heq]. split; [| subst; auto].
+      exists []. split.
+      + exists []. split. apply is_indexed_elements_nil. split; [simpl; auto | intros; contradiction].
+      + subst. reflexivity.
   }
-  destruct H2 as [[s2 [Hfeas2 Hsum2]] Hmax2]. 
-  apply Z.max_case_strong; intros Hle. 
+  destruct H2 as [[s2 [Hfeas2 Hsum2]] Hmax2].
+  apply Z.max_case_strong; intros Hle.
   - 
-    left.  exists s1. split; [| split].
-    + apply feasible_set_app_x_l.  assumption.
+    left. exists s1. split; [| split].
+    + apply feasible_set_app_x_l. assumption.
     + assumption.
     + intros t Ht.
       apply feasible_set_app_x_inv in Ht.
@@ -664,35 +669,35 @@ Proof.
       * 
         apply Hmax1. assumption.
       *
-        subst t.  rewrite sum_app.  simpl. rewrite Z.add_0_r. 
+        subst t. rewrite sum_app. simpl. rewrite Z.add_0_r.
         specialize (Hmax2 t' Ht').
         lia.
   - 
     left. exists (s2 ++ [x]). split; [| split].
     + apply feasible_set_app_x_r. assumption.
-    + rewrite sum_app. simpl.  rewrite Z.add_0_r. rewrite Hsum2. reflexivity.
+    + rewrite sum_app. simpl. rewrite Z.add_0_r. rewrite Hsum2. reflexivity.
     + intros t Ht.
       apply feasible_set_app_x_inv in Ht.
-      destruct Ht as [Ht | [t' [Heq Ht']]]. 
+      destruct Ht as [Ht | [t' [Heq Ht']]].
       * 
         specialize (Hmax1 t Ht). lia.
       * 
-        subst t. rewrite sum_app. simpl.  rewrite Z.add_0_r.
+        subst t. rewrite sum_app. simpl. rewrite Z.add_0_r.
         specialize (Hmax2 t' Ht').
         lia.
 Qed.
 
-Lemma removelast_app_x:  forall {A} (l:  list A) x,
+Lemma removelast_app_x: forall {A} (l: list A) x,
   removelast (l ++ [x]) = l.
 Proof.
   intros.
   rewrite removelast_app.
-  - simpl.  rewrite app_nil_r. reflexivity. 
+  - simpl. rewrite app_nil_r. reflexivity.
   - discriminate.
-Qed. 
+Qed.
 
-Lemma Hoare_list_iter {A B:  Type}:  
-  forall (body:  A -> B -> program B)
+Lemma Hoare_list_iter {A B: Type}: 
+  forall (body: A -> B -> program B)
          (l: list A)
          (default: B)
          (I: list A -> B -> Prop),
@@ -710,7 +715,7 @@ Proof.
             Hoare (list_iter body l_rest b_curr) 
                   (fun b_final => I (l_done ++ l_rest) b_final)).
   {
-    induction l_rest as [|x xs IH]. 
+    induction l_rest as [|x xs IH].
     - 
       intros b_curr l_done H_inv.
       simpl.
@@ -719,7 +724,7 @@ Proof.
       auto.
     - 
       intros b_curr l_done H_inv.
-      simpl. 
+      simpl.
       eapply Hoare_bind.
       + 
         apply H_step.
@@ -727,7 +732,7 @@ Proof.
       + 
         intros b_next H_next.
         specialize (IH b_next (l_done ++ [x]) H_next).
-        rewrite <- app_assoc in IH. 
+        rewrite <- app_assoc in IH.
         auto.
   }
   specialize (H_gen l default [] H_init).
@@ -736,14 +741,14 @@ Proof.
 Qed.
 
 (** Level 2: Prove that the algorithm returns the correct maximum value *)
-Theorem max_sum_value_correct : 
+Theorem max_sum_value_correct :
   forall l,
     Hoare (max_sum l)
       (fun '(m, _) => max_value_spec l m).
 Proof.
   intros l.
-  unfold max_sum. 
-  eapply Hoare_bind.  
+  unfold max_sum.
+  eapply Hoare_bind. 
   - eapply Hoare_list_iter with 
       (I := fun done st => 
               match st with 
@@ -752,31 +757,31 @@ Proof.
                   max_value_spec (removelast done) m2
               end).
     + 
-      simpl.  split; apply max_value_spec_nil.  
+      simpl. split; apply max_value_spec_nil. 
     + 
-      intros x done st. 
+      intros x done st.
       destruct st as [[[m1 ans1] m2] ans2].
-      intros [Hm1 Hm2].  
-      apply Hoare_choice.  
+      intros [Hm1 Hm2]. 
+      apply Hoare_choice. 
       *
-        eapply Hoare_assume_bind.  
-        intros H_le.  
-        apply Hoare_ret.   
-        split.  
+        eapply Hoare_assume_bind. 
+        intros H_le. 
+        apply Hoare_ret.  
+        split. 
         -- 
-           assert (Hmax:  max_value_spec (done ++ [x]) (Z.max m1 (m2 + x))).
+           assert (Hmax: max_value_spec (done ++ [x]) (Z.max m1 (m2 + x))).
            { apply max_value_spec_app; auto. }
            replace (Z.max m1 (m2 + x)) with (m2 + x) in Hmax.
-           ++ exact Hmax.  
-           ++ symmetry. apply Z.max_r. lia.  
+           ++ exact Hmax. 
+           ++ symmetry. apply Z.max_r. lia. 
         --
            rewrite removelast_app_x.
            auto.
       *
         eapply Hoare_assume_bind. 
         intros H_ge. 
-        apply Hoare_ret.  
-        split.   
+        apply Hoare_ret. 
+        split.  
         -- 
            assert (Hmax: max_value_spec (done ++ [x]) (Z.max m1 (m2 + x))).
            { apply max_value_spec_app; auto. }
@@ -787,21 +792,21 @@ Proof.
            rewrite removelast_app_x.  
            auto.  
   -
-    intros st.  destruct st as [[[m1 ans1] m2] ans2].
-    intros [Hm1 _].   
+    intros st. destruct st as [[[m1 ans1] m2] ans2].
+    intros [Hm1 _].  
     apply Hoare_ret.  
     exact Hm1.
-Qed.  
+Qed. 
 
 (** Level 3: Prove that the algorithm returns a correct feasible subsequence achieving the maximum value *)
-Lemma sum_single:  forall x, sum [x] = x.
-Proof.  intros. simpl. apply Z.add_0_r.  Qed.
+Lemma sum_single: forall x, sum [x] = x.
+Proof. intros. simpl. apply Z.add_0_r. Qed.
 
-Lemma sincr_tail:  forall a l, sincr (a :: l) -> sincr l.
-Proof. 
-  intros a l Hsincr.  unfold sincr in *.
-  destruct l as [|b l']. 
-  - simpl.  auto.
+Lemma sincr_tail: forall a l, sincr (a :: l) -> sincr l.
+Proof.
+  intros a l Hsincr. unfold sincr in *.
+  destruct l as [|b l'].
+  - simpl. auto.
   - simpl in Hsincr. simpl. inversion Hsincr; subst. assumption.
 Qed.   
 
@@ -813,15 +818,15 @@ Proof.
   exists il. split; [| split; auto].
   - revert s l t Hsincr Hgap Hidx.  
     induction il as [|i il' IH]; intros s l t Hsincr Hgap Hidx.
-    + inversion Hidx; subst.  apply Forall2_nil. 
+    + inversion Hidx; subst. apply Forall2_nil.
     + destruct t as [|y t'].
-      * inversion Hidx. 
-      * constructor. 
+      * inversion Hidx.
+      * constructor.
         -- inversion Hidx; subst.
            assert (H_range: 0 <= i < Zlength l).
-           { apply Znth_error_range in H2.  tauto. }
+           { apply Znth_error_range in H2. tauto. }
            rewrite (Znth_error_app_l _ _ _ H_range). apply H2.
-        -- inversion Hidx; subst.  apply IH.  
+        -- inversion Hidx; subst. apply IH. 
            ++ apply (sincr_tail i il' Hsincr).
            ++ intros i0 j0 Hi0 Hj0. apply Hgap.
               ** right. apply Hi0.
@@ -829,65 +834,65 @@ Proof.
            ++ apply H4.                
 Qed.
 
-Lemma last_In:  
-  forall (l:  list Z) (tail: Z),
+Lemma last_In: 
+  forall (l: list Z) (tail: Z),
     l <> [] -> In (last l tail) l.
 Proof. 
-  intros l tail H.  induction l as [|a l' IH]. 
-  - contradiction. 
+  intros l tail H. induction l as [|a l' IH].
+  - contradiction.
   - destruct l' as [|a' l''].
-    + simpl.  left. reflexivity.
-    + simpl.  right. apply IH. discriminate.
+    + simpl. left. reflexivity.
+    + simpl. right. apply IH. discriminate.
 Qed.         
 
-Lemma feasible_set_extend: 
+Lemma feasible_set_extend:
   forall (l: list Z) (s: Z) (t: list Z),
     feasible_set (removelast l) t -> 
     feasible_set (l ++ [s]) (t ++ [s]).
 Proof.
-  intros l s t Hfeas.  unfold feasible_set, non_adjacent_subseq in Hfeas.
-  destruct Hfeas as [il [Hidx [Hsincr Hgap]]]. 
-  exists (il ++ [Zlength l]). repeat split.  
+  intros l s t Hfeas. unfold feasible_set, non_adjacent_subseq in Hfeas.
+  destruct Hfeas as [il [Hidx [Hsincr Hgap]]].
+  exists (il ++ [Zlength l]). repeat split. 
   - apply is_indexed_elements_app.
-    + apply is_indexed_elements_extend.  apply Hidx.
-    + apply is_indexed_elements_cons. 
-      * apply Znth_error_snoc_last. 
+    + apply is_indexed_elements_extend. apply Hidx.
+    + apply is_indexed_elements_cons.
+      * apply Znth_error_snoc_last.
       * apply is_indexed_elements_nil.
-  - apply sincr_extend_last. 
-    + apply Hsincr. 
+  - apply sincr_extend_last.
+    + apply Hsincr.
     + destruct il as [|i' il'].
-      * left. reflexivity.  
-      * right. apply is_indexed_elements_range in Hidx.  
+      * left. reflexivity. 
+      * right. apply is_indexed_elements_range in Hidx. 
         rewrite Forall_forall in Hidx.
         assert (Hlast_In: In(last (i' :: il') 0) (i' :: il')).
         { apply last_In. discriminate. }
         specialize (Hidx _ Hlast_In).
         destruct (list_snoc_destruct l) as [Heq_l | [a [l' Heq_l]]].
-        -- subst l; simpl in *; unfold Zlength in *; simpl in *.  lia.
-        -- subst l.  rewrite removelast_app in Hidx by discriminate. 
+        -- subst l; simpl in *; unfold Zlength in *; simpl in *. lia.
+        -- subst l. rewrite removelast_app in Hidx by discriminate.
            simpl in Hidx. rewrite app_nil_r in Hidx.
-           rewrite Zlength_app.  unfold Zlength in *.  simpl.  lia.
+           rewrite Zlength_app. unfold Zlength in *.  simpl. lia.
   - intros x y Hx Hy. apply in_app_or in Hx. apply in_app_or in Hy.
     destruct Hx as [Hx_il | Hx_lt]; destruct Hy as [Hy_il | Hy_lt].
     + apply Hgap; tauto.
-    + simpl in *. destruct Hy_lt as [Heq_y | Hf]; [|contradiction]. 
-      subst y. apply is_indexed_elements_range in Hidx. 
-      rewrite Forall_forall in Hidx.  specialize (Hidx _ Hx_il).
+    + simpl in *. destruct Hy_lt as [Heq_y | Hf]; [|contradiction].
+      subst y. apply is_indexed_elements_range in Hidx.
+      rewrite Forall_forall in Hidx. specialize (Hidx _ Hx_il).
       destruct (list_snoc_destruct l) as [Heq_l | [a [l' Heq_l]]].
-      * subst l.  simpl in Hidx. unfold Zlength in *. simpl.  lia.
-      * subst l. rewrite removelast_app in Hidx by discriminate. 
-        simpl in Hidx. rewrite app_nil_r in Hidx.
-        rewrite Zlength_app. unfold Zlength in *. simpl. lia. 
-    + simpl in *. destruct Hx_lt as [Heq_x | Hf]; [|contradiction].  
-      subst x. apply is_indexed_elements_range in Hidx.  
-      rewrite Forall_forall in Hidx.  specialize (Hidx _ Hy_il). 
-      destruct (list_snoc_destruct l) as [Heq_l | [a [l' Heq_l]]].  
-      * subst l.  simpl.  unfold Zlength in *.  simpl in *. lia.
+      * subst l. simpl in Hidx. unfold Zlength in *. simpl. lia.
       * subst l. rewrite removelast_app in Hidx by discriminate.
-        simpl in Hidx. rewrite app_nil_r in Hidx.  
+        simpl in Hidx. rewrite app_nil_r in Hidx.
+        rewrite Zlength_app. unfold Zlength in *. simpl. lia.
+    + simpl in *. destruct Hx_lt as [Heq_x | Hf]; [|contradiction]. 
+      subst x. apply is_indexed_elements_range in Hidx. 
+      rewrite Forall_forall in Hidx. specialize (Hidx _ Hy_il). 
+      destruct (list_snoc_destruct l) as [Heq_l | [a [l' Heq_l]]]. 
+      * subst l. simpl. unfold Zlength in *. simpl in *. lia.
+      * subst l. rewrite removelast_app in Hidx by discriminate.
+        simpl in Hidx. rewrite app_nil_r in Hidx. 
         rewrite Zlength_app. unfold Zlength in *. simpl. lia.
     + simpl in *. destruct Hx_lt as [Heq_x | Hf]; [|contradiction].
-      destruct Hy_lt as [Heq_y | Hf]; [|contradiction]. subst x y.  lia.    
+      destruct Hy_lt as [Heq_y | Hf]; [|contradiction]. subst x y. lia.    
 Qed.
 
 Theorem max_sum_full_correct :
@@ -895,7 +900,7 @@ Theorem max_sum_full_correct :
     Hoare (max_sum l)
       (fun '(m, s) => max_sum_full_spec l m s).
 Proof.
-  intros l.  unfold max_sum.  eapply Hoare_bind. 
+  intros l. unfold max_sum. eapply Hoare_bind.
   - eapply Hoare_list_iter with 
       (I := fun done st => 
               match st with 
@@ -909,778 +914,1300 @@ Proof.
       * apply max_value_spec_nil.
       * apply max_value_spec_nil.
       * apply feasible_set_nil_intro.
-      * apply feasible_set_nil_intro. 
-    + intros x done st.  destruct st as [[[m1 ans1] m2] ans2].
-      intros [Hm1 [Hm2 [Hfeas1 [Hsum1 [Hfeas2 Hsum2]]]]].  apply Hoare_choice.
-      * eapply Hoare_assume_bind. intros H_le. apply Hoare_ret.  repeat split.  
+      * apply feasible_set_nil_intro.
+    + intros x done st. destruct st as [[[m1 ans1] m2] ans2].
+      intros [Hm1 [Hm2 [Hfeas1 [Hsum1 [Hfeas2 Hsum2]]]]]. apply Hoare_choice.
+      * eapply Hoare_assume_bind. intros H_le. apply Hoare_ret. repeat split. 
         -- assert (Hmax: max_value_spec (done ++ [x]) (Z.max m1 (m2 + x))).
            { apply max_value_spec_app; auto. }
            replace (Z.max m1 (m2 + x)) with (m2 + x) in Hmax.
-           ++ apply Hmax. 
+           ++ apply Hmax.
            ++ symmetry. apply Z.max_r. lia.
-        -- rewrite removelast_app_x.  apply Hm1.
-        -- apply feasible_set_extend.  tauto.
+        -- rewrite removelast_app_x. apply Hm1.
+        -- apply feasible_set_extend. tauto.
         -- simpl. rewrite sum_app, sum_single, Hsum2. reflexivity.
         -- rewrite removelast_app_x. apply Hfeas1.
         -- apply Hsum1.
-      * eapply Hoare_assume_bind. intros H_ge. apply Hoare_ret. repeat split. 
+      * eapply Hoare_assume_bind. intros H_ge. apply Hoare_ret. repeat split.
         -- assert (Hmax: max_value_spec (done ++ [x]) (Z.max m1 (m2 + x))).
            { apply max_value_spec_app; auto. }
-           replace (Z.max m1 (m2 + x)) with m1 in Hmax. 
-           ++ apply Hmax. 
+           replace (Z.max m1 (m2 + x)) with m1 in Hmax.
+           ++ apply Hmax.
            ++ symmetry. apply Z.max_l. lia.
         -- rewrite removelast_app_x. apply Hm1.
-        -- apply feasible_set_preserved.  assumption.
-        -- assumption. 
+        -- apply feasible_set_preserved. assumption.
+        -- assumption.
         -- rewrite removelast_app_x. apply Hfeas1.
         -- apply Hsum1.
-  - intros st. destruct st as [[[m1 ans1] m2] ans2]. 
+  - intros st. destruct st as [[[m1 ans1] m2] ans2].
     intros [Hm1 [Hm2 [Hfeas1 [Hsum1 [_ _]]]]]. apply Hoare_ret.
-    unfold max_sum_full_spec. repeat split; auto. 
+    unfold max_sum_full_spec. repeat split; auto.
 Qed.
 
-(** ========================================================================
-    Level 4: Lexicographically minimal solution
-    ======================================================================== *)
-
-Definition nat_list_to_Z_list (l: list nat) : list Z := map Z.of_nat l.
-
 (** Lexicographical comparison of index lists *)
-Fixpoint index_lex_lt (il1 il2: list nat) : Prop :=
+Fixpoint index_lex_lt (il1 il2: list Z) : Prop :=
   match il1, il2 with
-  | [], [] => False           
-  | [], _ ::  _ => True      
+  | [], [] => False
+  | [], _ :: _ => True
   | _ :: _, [] => False
   | i1 :: il1', i2 :: il2' =>
-      (i1 < i2)%nat \/ (i1 = i2 /\ index_lex_lt il1' il2')
+      i1 < i2 \/ (i1 = i2 /\ index_lex_lt il1' il2')
   end.
 
-Definition non_adjacent_in_nat (il:  list nat): Prop :=
-  let il_Z := nat_list_to_Z_list il in
-  non_adjacent_in il_Z.
-
-Definition is_indexed_elements_nat (l: list Z) (il: list nat) (s: list Z) : Prop :=
-  is_indexed_elements l (nat_list_to_Z_list il) s.
-
-Definition lex_min_spec (l: list Z) (m: Z) (s: list Z) (il: list nat) : Prop :=
+(** Specification for lexicographically minimal optimal solution *)
+(** We require that for any other optimal solution (s', il'), our il is lexicographically <= il' *)
+Definition lex_min_spec (l: list Z) (m: Z) (s: list Z) (il: list Z) : Prop :=
   max_sum_full_spec l m s /\
-  is_indexed_elements_nat l il s /\
-  non_adjacent_in_nat il /\
-  (forall s' (il':  list nat), 
+  is_indexed_elements l il s /\
+  non_adjacent_in il /\
+  (forall s' il', 
      feasible_set l s' -> 
-     is_indexed_elements_nat l il' s' -> 
-     non_adjacent_in_nat il' ->
+     is_indexed_elements l il' s' -> 
+     non_adjacent_in il' ->
      sum s' = m -> 
      index_lex_lt il il' \/ il = il').
 
 (** Modified algorithm to find the lexicographically minimal solution *)
-Definition max_sum_lex (l: list Z): program (Z * list Z * list nat) :=
+Definition max_sum_lex (l: list Z): program (Z * list Z * list Z) :=
   '(max1, ans1, il1, _, _, _, _) <- 
     list_iter
       (fun n =>
          fun '(max1, ans1, il1, max2, ans2, il2, idx) =>
-           let sum_include := max2 + n in
            choice
-             (assume (sum_include > max1);; 
-              ret (sum_include, ans2 ++ [n], il2 ++ [idx], max1, ans1, il1, (idx + 1)%nat))
+             (assume (max2 + n > max1);; 
+              ret (max2 + n, ans2 ++ [n], il2 ++ [idx], max1, ans1, il1, idx + 1))
              (choice
-                (assume (sum_include < max1);;
-                 ret (max1, ans1, il1, max1, ans1, il1, (idx + 1)%nat))
-                (assume (sum_include = max1);;
+                (assume (max2 + n < max1);;
+                 ret (max1, ans1, il1, max1, ans1, il1, idx + 1))
+                (assume (max2 + n = max1);;
                   choice 
                     (assume (index_lex_lt (il2 ++ [idx]) il1);;
-                     ret (sum_include, ans2 ++ [n], il2 ++ [idx], max1, ans1, il1, (idx + 1)%nat))
+                     ret (max2 + n, ans2 ++ [n], il2 ++ [idx], max1, ans1, il1, idx + 1))
                     (assume (~ index_lex_lt (il2 ++ [idx]) il1);;
-                     ret (max1, ans1, il1, max1, ans1, il1, (idx + 1)%nat))
+                     ret (max1, ans1, il1, max1, ans1, il1, idx + 1))
                 )
              )
       )
       l
-      (0, [], [], 0, [], [], 0%nat);; 
+      (0, [], [], 0, [], [], 0);; 
   ret (max1, ans1, il1).
 
-Lemma Zlength_removelast_lt:  forall {A} (l: list A),
-  l <> [] ->
-  Zlength (removelast l) < Zlength l.
+
+Definition max_sum_lex_inv (done : list Z)
+             (max1 : Z) (ans1 : list Z) (il1 : list Z)
+             (max2 : Z) (ans2 : list Z) (il2 : list Z)
+             (idx : Z) : Prop :=
+  Zlength done = idx /\
+  (* ans1 is optimal and lex-min for done *)
+  max_sum_full_spec done max1 ans1 /\
+  is_indexed_elements done il1 ans1 /\
+  non_adjacent_in il1 /\
+  (forall s' il',
+     feasible_set done s' ->
+     is_indexed_elements done il' s' ->
+     non_adjacent_in il' ->
+     sum s' = max1 ->
+     index_lex_lt il1 il' \/ il1 = il') /\
+  (* ans2 is optimal and lex-min for removelast done *)
+  (match done with
+   | [] => max2 = 0 /\ ans2 = [] /\ il2 = []
+   | _ => max_sum_full_spec (removelast done) max2 ans2 /\
+          is_indexed_elements (removelast done) il2 ans2 /\
+          non_adjacent_in il2 /\
+          (forall s' il',
+             feasible_set (removelast done) s' ->
+             is_indexed_elements (removelast done) il' s' ->
+             non_adjacent_in il' ->
+             sum s' = max2 ->
+             index_lex_lt il2 il' \/ il2 = il')
+   end).
+
+Definition all_positive (l:  list Z): Prop :=
+  Forall (fun x => x > 0) l.
+
+Lemma proof_il'_nil :
+  forall (s' il' : list Z)
+    (H : feasible_set [] s')
+    (H0 : is_indexed_elements [] il' s')
+    (H1 : non_adjacent_in il')
+    (H2 : sum s' = 0),
+    [] = il'.
 Proof.
-  intros A l Hneq. 
-  destruct l using rev_ind.
-  - contradiction. 
-  - rewrite removelast_app_x. 
-    rewrite Zlength_app. 
-    assert (Zlength [x] = 1).
-    { unfold Zlength. simpl. auto. }
-    lia. 
+  intros s' il' H H0 H1 H2.
+  apply feasible_set_nil in H.
+  subst s'.
+  apply is_indexed_elements_nil_inv_r in H0.
+  rewrite H0; reflexivity.
 Qed.
 
-Lemma sincr_app_singleton: forall (il: list Z) (x: Z),
-  sincr il ->
-  (forall i, In i il -> i < x) ->
-  sincr (il ++ [x]).
+Lemma idx_eq_zero (idx : Z) (Hlen : Zlength ([] : list Z) = idx) : idx = 0.
 Proof.
-  intros il x Hsincr Hbound.
-  induction il as [| a il' IH].
-  - simpl. auto.
-  - simpl.  destruct il' as [| b il''].
-    + simpl.  simpl in Hsincr. split; auto.
-      apply Hbound.  left. reflexivity.
-    + simpl in Hsincr. destruct Hsincr as [Hab Hrest].
-      simpl. split; [assumption |].
-      apply IH; [assumption |]. 
-      intros i Hi. apply Hbound. right. assumption.
+  unfold Zlength in Hlen.
+  simpl in Hlen.
+  rewrite Hlen; reflexivity.
 Qed.
 
-Lemma index_lex_lt_or_eq: forall il1 il2,
-  index_lex_lt il1 il2 \/ il1 = il2 \/ index_lex_lt il2 il1.
-Proof. 
-  intros il1.
-  induction il1 as [| a1 il1' IH]; intros il2.
-  - destruct il2 as [| a2 il2'].
-    + right. left. reflexivity.
-    + left. simpl. auto.
-  - destruct il2 as [| a2 il2'].
-    + right. right. simpl. auto.
-    + simpl. 
-      destruct (Nat.lt_trichotomy a1 a2) as [Hlt | [Heq | Hgt]].
-      * left. left. exact Hlt.
-      * subst a2.
-        specialize (IH il2').
-        destruct IH as [IH_lt | [IH_eq | IH_gt]].
-        -- left. right. split; [reflexivity | exact IH_lt]. 
-        -- right. left. rewrite IH_eq. reflexivity.
-        -- right. right. right. split; [reflexivity | exact IH_gt].
-      * right. right. left. exact Hgt. 
+Lemma In_0_non_adjacent :
+  forall i j : Z, In i [0] -> In j [0] -> i + 1 <> j.
+Proof.
+  intros. destruct H, H0.
+  ++ lia.
+  ++ simpl in H0. tauto.
+  ++ simpl in H. tauto.
+  ++ simpl in H. tauto.
 Qed.
 
-Lemma is_indexed_elements_nat_length: 
-  forall l il s,
-    is_indexed_elements_nat l il s ->
-    length il = length s. 
+Lemma is_indexed_elements_restrict :
+  forall (l : list Z) (x : Z) (s il : list Z),
+  is_indexed_elements (l ++ [x]) il s ->
+  (forall i, In i il -> i < Zlength l) ->
+  is_indexed_elements l il s.
 Proof.
-  intros l il s H.
-  unfold is_indexed_elements_nat, nat_list_to_Z_list in H.
-  apply Forall2_length in H.
-  rewrite map_length in H. 
-  exact H.
-Qed. 
-
-Lemma positive_sum_ge_length:
-  forall s,
-    Forall (fun x => x > 0) s ->
-    sum s >= Z.of_nat (length s).
-Proof.
-  intros s Hpos.
-  induction s as [| h t IH].
-  - simpl.   lia.
-  - simpl.  
-    rewrite Forall_cons_iff in Hpos.
-    destruct Hpos as [Hh Ht].
-    specialize (IH Ht).
-    unfold sum in *. simpl.
-    lia.
-Qed.
-
-Lemma feasible_set_elements_from_source:
-  forall l s,
-    feasible_set l s ->
-    Forall (fun x => In x l) s.
-Proof.
-  intros l s Hfeas.
-  unfold feasible_set, non_adjacent_subseq in Hfeas.
-  destruct Hfeas as [il [Hidx _]].
+  intros l x s il Hidx Hbound.
   revert s Hidx.
-  induction il as [| i il' IH]; intros s Hidx. 
-  - apply is_indexed_elements_nil_inv_l in Hidx.  subst.  apply Forall_nil. 
-  -
-    apply is_indexed_elements_cons_inv_l in Hidx. 
-    destruct Hidx as [a [s' [Hnth [Hidx' Heq_s]]]].
-    subst s. 
-    apply Forall_cons.
-    + unfold Znth_error in Hnth. 
-      destruct (Z_le_gt_dec 0 i).
-      * apply nth_error_In in Hnth.  exact Hnth.
-      * discriminate.
-    + apply IH.   exact Hidx'. 
+  induction il as [|i il' IH]; intros s Hidx; simpl in *.
+  - apply is_indexed_elements_nil_inv_l in Hidx.
+    rewrite Hidx.
+    apply is_indexed_elements_nil.
+  - apply is_indexed_elements_cons_inv_l in Hidx as (a & s' & Hnth & Hrest & ->).
+    apply is_indexed_elements_cons.
+    + (* Goal: Znth_error l i = Some a *)
+      (* From Hnth: Znth_error (l ++ [x]) i = Some a *)
+      pose proof (Znth_error_range _ _ _ Hnth) as [Hge Hlt_full].
+      (* Hbound gives: i < Zlength l *)
+      assert (Hin: In i (i :: il')) by (left; reflexivity).
+      specialize (Hbound i Hin) as Hlt.
+      (* Now we have 0 <= i and i < Zlength l *)
+      rewrite (Znth_error_app_l l [x] i (conj Hge Hlt)) in Hnth.
+      exact Hnth.
+    + (* Inductive step for il' *)
+      apply IH.
+      intros j Hj.
+      apply Hbound.
+      right. exact Hj. tauto.
 Qed.
 
-(** 辅助引理：index_lex_lt 在添加相同元素后保持（需要长度相等）*)
-Lemma index_lex_lt_app_same: 
-  forall il1 il2 idx,
-    length il1 = length il2 ->
-    index_lex_lt il1 il2 ->
-    index_lex_lt (il1 ++ [idx]) (il2 ++ [idx]).
+Lemma max_sum_full_spec_inv :
+  forall (l : list Z) (m : Z) (s : list Z),
+  max_sum_full_spec l m s ->
+  max_value_spec l m /\ feasible_set l s /\ sum s = m.
 Proof.
-  intros il1 il2 idx Hlen Hlt.
-  revert il2 idx Hlen Hlt.
-  induction il1 as [| h1 t1 IH]; intros il2 idx Hlen Hlt.
-  - destruct il2; simpl in *; try contradiction; try discriminate.
-  - destruct il2; simpl in *; try discriminate.
-    injection Hlen as Hlen'. 
-    destruct Hlt as [Hlt_h | [Heq_h Hlt_t]].
-    + left. exact Hlt_h. 
-    + right. split. 
-      * exact Heq_h.
-      * apply IH; assumption. 
+  intros l m s H.
+  exact H.
 Qed.
 
-(** 主定理：添加正数条件 *)
-Theorem max_sum_lex_correct:
+Lemma feasible_single :
+  forall x : Z,
+    feasible_set [x] [x].
+Proof.
+  unfold feasible_set, non_adjacent_subseq.
+  exists [0].
+  split.
+  + unfold is_indexed_elements.
+      constructor; [compute; reflexivity | constructor].
+  + unfold non_adjacent_in; simpl.
+    split; [tauto | intros i j Hi Hj; inversion Hi; inversion Hj; lia].
+Qed.
+
+Lemma Zlength_removelast : forall (A: Type) (l : list A),
+  l <> [] -> Zlength (removelast l) = Zlength l - 1.
+Proof.
+  intros A l Hnonnil.
+  induction l as [| a l'].
+  - exfalso; contradiction.
+  - destruct l' as [| b l''].
+    + simpl removelast. simpl. unfold Zlength. tauto.
+    + simpl removelast in *.
+      assert (Hl'_nonnil : b :: l'' <> []) by (
+        intros H; discriminate H
+      ).
+      rewrite Zlength_cons.
+      rewrite Zlength_cons.
+      rewrite (IHl' Hl'_nonnil).
+      lia.
+Qed.
+
+Lemma in_singleton: forall {A} (a x : A), In x [a] <-> x = a.
+Proof.
+  split; intros H.
+  - now inversion H.
+  - subst; left; reflexivity.
+Qed.
+
+
+Lemma max_value_spec_single_positive :
+  forall x : Z, x > 0 -> max_value_spec [x] x.
+Proof.
+  intros x Hx. left. exists [x]. repeat split.
+  - apply feasible_single.
+  - apply sum_single.
+  - intros t Ht. unfold feasible_set, non_adjacent_subseq in *.
+    destruct Ht as [il [Hidx Hnonadj]].
+    assert (Ht_is_empty_or_x: t = [] \/ t = [x]).
+    { 
+      unfold is_indexed_elements in Hidx. destruct t as [|a t'].
+      + left. auto.
+      + right. apply is_indexed_elements_cons_inv_r in Hidx.
+        destruct Hidx as [i [il' [Heq [Hnth Hrest]]]].
+        assert (Hi: i = 0).
+        { 
+          apply Znth_error_range in Hnth. unfold Zlength in Hnth. simpl in Hnth. lia. 
+        }
+        subst i. assert (Ha: a = x).
+        {
+          assert (Hx_nth: Znth_error [x] 0 = Some x) by apply Znth_error_cons_0. 
+          rewrite Hx_nth in Hnth. injection Hnth as Ha. symmetry. apply Ha.
+        }
+        subst a. assert (Ht'_nil: t' = []).
+        {
+          destruct t' as [|b t''].
+          - reflexivity. 
+          - exfalso. apply is_indexed_elements_cons_inv_r in Hrest.
+            destruct Hrest as [j [il'' [Heq_il' [Hnth' Hrest']]]].
+            apply Znth_error_range in Hnth'. simpl in Hnth'.
+            destruct Hnonadj as [Hsincr _]. rewrite Heq in Hsincr.
+            apply sincr_cons_tail_Forall_lt in Hsincr. rewrite Heq_il' in Hsincr.
+            assert (Hj_in: In j (j :: il'')) by (left;reflexivity).
+            assert (Hj_0: j = 0) by (unfold Zlength in Hnth'; simpl in Hnth'; lia).  
+            rewrite Hj_0 in Hsincr.
+            apply Forall_cons_iff in Hsincr.
+            destruct Hsincr as [H0 _].
+            lia.
+        }
+        rewrite Ht'_nil.
+        reflexivity. 
+    }
+    destruct Ht_is_empty_or_x.
+    + rewrite H; simpl; lia.
+    + rewrite H; simpl; lia.
+Qed.
+
+
+
+(* 此时 x>0, 取x最大 *)
+Lemma max_sum_lex_inv_single_positive :
+  forall (l : list Z) (x : Z)
+    (Hfull1 : max_sum_full_spec [] 0 [])
+    (Hgap1 : non_adjacent_in [])
+    (Hgt : x > 0)
+    (Hlex1 : forall s' il',
+               feasible_set [] s' ->
+               is_indexed_elements [] il' s' ->
+               non_adjacent_in il' -> sum s' = 0 ->
+               index_lex_lt [] il' \/ [] = il')
+    (Hidx0 : Zlength ([] : list Z) = 0),
+  max_sum_lex_inv [x] x [x] [0] 0 [] [] 1.
+Proof.
+  intros l x Hfull1 Hgap1 Hgt Hlex1 Hidx0.
+  unfold max_sum_lex_inv.
+  repeat split.
+  - apply max_value_spec_single_positive; tauto.
+  - apply feasible_single.
+  - apply sum_single.
+  - (* is_indexed_elements [x] [0] [x] *)
+    unfold is_indexed_elements.
+    apply Forall2_cons.
+    + simpl; reflexivity.
+    + apply Forall2_nil.
+  - apply In_0_non_adjacent.
+  - intros s' il' Hfeas Hidx Hnonadj Hsum.
+    change ([x]) with ([] ++ [x]) in Hfeas.
+    apply feasible_set_app_x_inv in Hfeas as [Hl | [t' [Heq Ht']]].
+    + exfalso. apply feasible_set_nil in Hl; subst s'. simpl in Hsum. lia.
+    + subst s'. apply feasible_set_nil in Ht'; subst t'.
+      simpl in Hidx.
+      apply is_indexed_elements_cons_inv_r in Hidx.
+      destruct Hidx as (i & il'' & Heq_il & Hnth & Hnil).
+      subst il'.
+      apply is_indexed_elements_nil_inv_r in Hnil; subst il''.
+      apply Znth_error_range in Hnth.
+      simpl in Hnth. assert (i = 0). { destruct Hnth; unfold Zlength in H0; simpl in H0; lia. }
+      subst i.
+      right. reflexivity.
+  - simpl. apply max_value_spec_nil.
+  - simpl. apply feasible_set_nil_intro.
+  - simpl. apply is_indexed_elements_nil.
+  - tauto.
+  - apply Hlex1.
+Qed.
+
+(* 此时 x < max1 = 0, 不取就是最大 *)
+Lemma max_sum_lex_inv_single_case :
+  forall (l : list Z) (x max1 idx : Z) (ans1 il1 : list Z)
+    (Hlen : Zlength ([] : list Z) = idx)
+    (Hfull1 : max_sum_full_spec [] max1 ans1)
+    (Hidx1 : is_indexed_elements [] il1 ans1)
+    (Hgap1 : non_adjacent_in il1)
+    (Hlex1 : forall s' il',
+               feasible_set [] s' ->
+               is_indexed_elements [] il' s' ->
+               non_adjacent_in il' -> sum s' = max1 ->
+               index_lex_lt il1 il' \/ il1 = il')
+    (Hlt : x < max1),
+  max_sum_lex_inv [x] max1 ans1 il1 max1 ans1 il1 (idx + 1).
+Proof.
+  intros l x max1 idx ans1 il1 Hlen Hfull1 Hidx1 Hgap1 Hlex1 Hlt.
+  unfold max_sum_lex_inv.
+  repeat split.
+
+  - simpl in Hlen; unfold Zlength in Hlen; simpl in Hlen; rewrite <- Hlen; reflexivity.
+  - pose proof (proj1 (proj2 Hfull1)) as Hfeas_ans.
+    pose proof (proj2 (proj2 Hfull1)) as Hsum_ans.
+    apply feasible_set_nil in Hfeas_ans. rewrite Hfeas_ans in Hsum_ans.
+    simpl in Hsum_ans.  (* Hsum_ans : 0 = max1 *)
+    subst max1.
+    (* Now prove max_value_spec [x] 0 *)
+    right.
+    split.
+    + intros s Hfeas.
+      change ([x]) with ([] ++ [x]) in Hfeas.
+      apply feasible_set_app_x_inv in Hfeas as [Hl | [t' [Heq Ht']]].
+      * (* s feasible in [] => s = [] => sum = 0 *)
+        apply feasible_set_nil in Hl; subst s; simpl; lia.
+      * (* s = t' ++ [x], t' feasible in [] => t' = [], s = [x] *)
+        apply feasible_set_nil in Ht'; subst t'. simpl in Heq; subst s.
+        simpl. lia.  (* x < 0, so sum = x < 0 <= 0 *)
+    + reflexivity.
+  - (* feasible_set [x] ans1 *)
+    apply max_sum_full_spec_inv in Hfull1 as [_ [Hfeas _]].
+    apply feasible_set_nil in Hfeas; subst ans1.
+    unfold feasible_set. unfold non_adjacent_subseq. exists []. split.
+    * apply is_indexed_elements_nil.
+    * unfold non_adjacent_in. split.
+      -- unfold sincr. tauto.
+      -- intros i j Hini Hinj. destruct Hini, Hinj.
+  - apply (proj2 (proj2 Hfull1)).
+  - (* is_indexed_elements [x] il1 ans1 *)
+    apply max_sum_full_spec_inv in Hfull1 as [_ [Hfeas _]].
+    apply feasible_set_nil in Hfeas; subst ans1.
+    apply is_indexed_elements_nil_inv_r in Hidx1; subst il1.
+    apply is_indexed_elements_nil.
+  - apply (proj1 Hgap1).
+  - apply (proj2 Hgap1).
+  - (* lex min for [x] *)
+    intros s' il' Hfeas Hidx Hnonadj Hsum.
+    (* Extract ans1 = [], max1 = 0 *)
+    pose proof (proj1 (proj2 Hfull1)) as Hfeas_ans.
+    pose proof (proj2 (proj2 Hfull1)) as Hsum_ans.
+    apply feasible_set_nil in Hfeas_ans; subst ans1.
+    simpl in Hsum_ans.  (* Hsum_ans : 0 = max1 *)
+    rewrite <- Hsum_ans in Hsum.   (* sum s' = 0 *)
+    rewrite <- Hsum_ans in Hlt.    (* x < 0 *)
+    change ([x]) with ([] ++ [x]) in Hfeas.
+    apply feasible_set_app_x_inv in Hfeas as [Hl | [t' [Heq Ht']]].
+    + (* s' = [] *)
+      apply feasible_set_nil in Hl; subst s'.
+      apply is_indexed_elements_nil_inv_r in Hidx; subst il'.
+      apply is_indexed_elements_nil_inv_r in Hidx1; subst il1.
+      right. reflexivity.
+    + (* s' = t' ++ [x] *)
+      apply feasible_set_nil in Ht'; subst t'.
+      subst s'. simpl in Hsum.  (* Hsum : x = 0 *)
+      lia.  (* x = 0 and x < 0 → contradiction *)
+  - (* max_value_spec [] max1 *)
+    simpl. apply (proj1 Hfull1).
+  - (* feasible_set [] ans1 *)
+    apply (proj1 (proj2 Hfull1)).
+  - (* sum ans1 = max1 *)
+    apply (proj2 (proj2 Hfull1)).
+  - (* is_indexed_elements [] il1 ans1 *)
+    apply Hidx1.
+  - (* sincr il1 *)
+    apply (proj1 Hgap1).
+  - (* non-adjacent gap *)
+    apply (proj2 Hgap1).
+  - (* lex min for [] *)
+    apply Hlex1.
+Qed.
+
+(* Hlt 矛盾 *)
+Lemma max_sum_lex_inv_contradiction_case :
+  forall (l : list Z) (x max1 idx : Z) (ans1 il1 : list Z)
+    (Hlen : Zlength ([] : list Z) = idx)
+    (Hfull1 : max_sum_full_spec [] max1 ans1)
+    (Hidx1 : is_indexed_elements [] il1 ans1)
+    (Hgap1 : non_adjacent_in il1)
+    (Hlex1 : forall s' il',
+               feasible_set [] s' ->
+               is_indexed_elements [] il' s' ->
+               non_adjacent_in il' -> sum s' = max1 ->
+               index_lex_lt il1 il' \/ il1 = il')
+    (Heq : x = max1)
+    (Hlt : index_lex_lt ([] ++ [idx]) il1),
+  max_sum_lex_inv [x] x [x] [idx] max1 ans1 il1 (idx + 1).
+Proof.
+  intros l x max1 idx ans1 il1 Hlen Hfull1 Hidx1 Hgap1 Hlex1 Heq Hlt.
+  unfold max_sum_lex_inv.
+  repeat split.
+
+  - simpl in Hlen; unfold Zlength in Hlen; simpl in Hlen; rewrite <- Hlen; reflexivity.
+  - pose proof (proj1 (proj2 Hfull1)) as Hfeas_ans.
+    pose proof (proj2 (proj2 Hfull1)) as Hsum_ans.
+    apply feasible_set_nil in Hfeas_ans. rewrite Hfeas_ans in Hsum_ans.
+    simpl in Hsum_ans.  (* Hsum_ans : 0 = max1 *)
+    subst max1.
+    (* Now prove max_value_spec [x] 0 *)
+    right.
+    split.
+    + intros s Hfeas.
+      change ([x]) with ([] ++ [x]) in Hfeas.
+      apply feasible_set_app_x_inv in Hfeas as [Hl | [t' [Heq Ht']]].
+      * (* s feasible in [] => s = [] => sum = 0 *)
+        apply feasible_set_nil in Hl; subst s; simpl; lia.
+      * (* s = t' ++ [x], t' feasible in [] => t' = [], s = [x] *)
+        apply feasible_set_nil in Ht'; subst t'. simpl in Heq; subst s.
+        simpl. lia.  (* x < 0, so sum = x < 0 <= 0 *)
+    + rewrite Hsum_ans. reflexivity.
+  - apply feasible_single.
+  - apply sum_single.
+  - unfold is_indexed_elements.
+    simpl in Hlen; unfold Zlength in Hlen; simpl in Hlen.
+    constructor.
+    + rewrite <- Hlen. reflexivity.
+    + constructor.
+  - intros i j Hini Hinj. destruct Hini, Hinj.
+    + lia.
+    + simpl in H0; tauto.
+    + simpl in H; tauto.
+    + simpl in H; tauto.
+  - intros s' il' Hfeas Hidx Hnonadj Hsum.
+    (* First, get ans1 = [] *)
+    pose proof (proj1 (proj2 Hfull1)) as Hfeas_ans.
+    apply feasible_set_nil in Hfeas_ans; subst ans1.
+    change ([x]) with ([] ++ [x]) in Hfeas.
+    apply feasible_set_app_x_inv in Hfeas as [Hl | [t' [Heq_s Ht']]].
+    + (* s' = [] *)
+      apply feasible_set_nil in Hl; subst s'.
+      apply is_indexed_elements_nil_inv_r in Hidx; subst il'.
+      (* Now Hidx1 : is_indexed_elements [] il1 [] *)
+      apply is_indexed_elements_nil_inv_r in Hidx1; subst il1.
+      left. exact Hlt.
+    + (* s' = [x] *)
+      pose proof (proj2 (proj2 Hfull1)) as Hsum_ans.
+      simpl in Hsum_ans. rewrite <- Heq in Hsum_ans.  (* x = 0 *)
+      apply feasible_set_nil in Ht'; subst t'. subst s'.
+      apply is_indexed_elements_cons_inv_r in Hidx.
+      destruct Hidx as (i & il'' & Heq_il & Hnth & Hnil).
+      subst il'.
+      apply is_indexed_elements_nil_inv_r in Hnil; subst il''.
+      apply Znth_error_range in Hnth.
+      simpl in Hnth. assert (i = 0). { destruct Hnth; unfold Zlength in H0; simpl in H0; lia. }
+      subst i.
+      simpl in Hlen; unfold Zlength in Hlen; simpl in Hlen.
+      rewrite Hlen.
+      right. reflexivity.
+- simpl. apply (proj1 Hfull1).
+- apply (proj1 (proj2 Hfull1)).
+- apply (proj2 (proj2 Hfull1)).
+- apply Hidx1.
+- apply (proj1 Hgap1).
+- apply (proj2 Hgap1).
+- apply Hlex1.
+Qed.
+
+Lemma max_sum_lex_inv_valid_case :
+  forall (l : list Z) (x max1 idx : Z) (ans1 il1 : list Z)
+    (Hlen : Zlength ([] : list Z) = idx)
+    (Hfull1 : max_sum_full_spec [] max1 ans1)
+    (Hidx1 : is_indexed_elements [] il1 ans1)
+    (Hgap1 : non_adjacent_in il1)
+    (Hlex1 : forall s' il',
+               feasible_set [] s' ->
+               is_indexed_elements [] il' s' ->
+               non_adjacent_in il' -> sum s' = max1 ->
+               index_lex_lt il1 il' \/ il1 = il')
+    (Heq : x = max1)
+    (Hnlt : ~ index_lex_lt ([] ++ [idx]) il1),
+  max_sum_lex_inv [x] max1 ans1 il1 max1 ans1 il1 (idx + 1).
+Proof.
+  intros l x max1 idx ans1 il1 Hlen Hfull1 Hidx1 Hgap1 Hlex1 Heq Hnlt.
+  unfold max_sum_lex_inv.
+  repeat split.
+  - simpl in Hlen; unfold Zlength in Hlen; simpl in Hlen; rewrite <- Hlen; reflexivity.
+  - pose proof (proj1 (proj2 Hfull1)) as Hfeas.
+    pose proof (proj2 (proj2 Hfull1)) as Hsum.
+    apply feasible_set_nil in Hfeas.
+    subst ans1.
+    simpl in Hsum.
+    subst max1.
+    right; split.
+    + intros s Hfeas_s.
+      change ([x]) with ([] ++ [x]) in Hfeas_s.
+      apply feasible_set_app_x_inv in Hfeas_s as [Hl | [t' [Heq Ht']]].
+      * apply feasible_set_nil in Hl; subst s; simpl; lia.
+      * apply feasible_set_nil in Ht'; subst t'; subst s; simpl; lia.
+    + rewrite Hsum; reflexivity.
+  - (* Goal 3: feasible_set [x] ans1 *)
+    pose proof (proj1 (proj2 Hfull1)) as Hfeas.
+    apply feasible_set_nil in Hfeas; subst ans1.
+    unfold feasible_set. unfold non_adjacent_subseq. exists []. split.
+    + apply is_indexed_elements_nil.
+    + unfold non_adjacent_in; split.
+      * unfold sincr; tauto.
+      * intros i j Hini Hinj. destruct Hini, Hinj.
+  - (* Goal 4: sum ans1 = max1 *)
+    pose proof (proj1 (proj2 Hfull1)) as Hfeas.
+    pose proof (proj2 (proj2 Hfull1)) as Hsum.
+    apply feasible_set_nil in Hfeas; subst ans1.
+    apply Hsum.
+  - (* Goal 5: is_indexed_elements [x] il1 ans1 *)
+    pose proof (proj1 (proj2 Hfull1)) as Hfeas.
+    apply feasible_set_nil in Hfeas. subst ans1.
+    apply is_indexed_elements_nil_inv_r in Hidx1. subst il1.
+    apply is_indexed_elements_nil.
+  - (* Goal 6: sincr il1 *)
+    pose proof (proj1 (proj2 Hfull1)) as Hfeas_ans.
+    apply feasible_set_nil in Hfeas_ans. subst ans1.
+    pose proof (proj2 (proj2 Hfull1)) as Hsum_ans. simpl in Hsum_ans. subst max1.
+    apply is_indexed_elements_nil_inv_r in Hidx1. subst il1. unfold sincr; tauto.
+  - (* Goal 7: gap condition *)
+    pose proof (proj1 (proj2 Hfull1)) as Hfeas_ans.
+    apply feasible_set_nil in Hfeas_ans. subst ans1.
+    apply is_indexed_elements_nil_inv_r in Hidx1; subst il1.
+    intros i j Hi Hj; contradiction.
+  - (* Goal 8: lex min for [x] *)
+    pose proof (proj1 (proj2 Hfull1)) as Hfeas.
+    pose proof (proj2 (proj2 Hfull1)) as Hsum.
+    apply feasible_set_nil in Hfeas; subst ans1.
+    simpl in Hsum; subst max1.
+    apply is_indexed_elements_nil_inv_r in Hidx1; subst il1.
+    intros s' il' Hfeas' Hidx' Hnonadj' Hsum'.
+    change ([x]) with ([] ++ [x]) in Hfeas'.
+    apply feasible_set_app_x_inv in Hfeas' as [Hl | [t' [Heq_s Ht']]].
+    + apply feasible_set_nil in Hl; subst s'.
+      apply is_indexed_elements_nil_inv_r in Hidx'; subst il'.
+      right; reflexivity.
+    + apply feasible_set_nil in Ht'; subst t'; subst s'.
+      apply is_indexed_elements_cons_inv_r in Hidx'.
+      destruct Hidx' as (i & il'' & -> & Hnth & Hnil).
+      apply is_indexed_elements_nil_inv_r in Hnil; subst il''.
+      apply Znth_error_range in Hnth.
+      assert (i = 0) by (destruct Hnth; unfold Zlength in *; simpl in *; lia).
+      subst i.
+      left; simpl; auto.
+  - (* Goal 9: max_value_spec (removelast [x]) max1 *)
+    pose proof (proj1 (proj2 Hfull1)) as Hfeas.
+    apply feasible_set_nil in Hfeas. subst ans1.
+    pose proof (proj2 (proj2 Hfull1)) as Hsum.
+    simpl in Hsum. subst max1.
+    assert (removelast [x] = []) by reflexivity. subst.
+    apply max_value_spec_nil.
+  - (* Goal 10: feasible_set (removelast [x]) ans1 *)
+    pose proof (proj1 (proj2 Hfull1)) as Hfeas.
+    apply feasible_set_nil in Hfeas; subst ans1.
+    apply feasible_set_nil_intro.
+  - (* Goal 11: sum ans1 = max1 *)
+    exact (proj2 (proj2 Hfull1)).
+  - (* Goal 12: is_indexed_elements (removelast [x]) il1 ans1 *)
+    pose proof (proj1 (proj2 Hfull1)) as Hfeas.
+    apply feasible_set_nil in Hfeas. subst ans1.
+    apply is_indexed_elements_nil_inv_r in Hidx1; subst il1.
+    pose proof (proj1 (proj2 Hfull1)) as Hfeas.
+    apply feasible_set_nil in Hfeas.
+    apply is_indexed_elements_nil.
+  - (* Goal 13: sincr il1 *)
+    pose proof (proj1 (proj2 Hfull1)) as Hfeas.
+    apply feasible_set_nil in Hfeas. subst ans1.
+    apply is_indexed_elements_nil_inv_r in Hidx1; subst il1.
+    simpl; auto.
+  - (* Goal 14: gap condition *)
+    pose proof (proj1 (proj2 Hfull1)) as Hfeas.
+    apply feasible_set_nil in Hfeas. subst ans1.
+    apply is_indexed_elements_nil_inv_r in Hidx1; subst il1.
+    intros i j Hi Hj; contradiction.
+  - (* Goal 15: lex min for removelast [x] = [] *)
+    pose proof (proj1 (proj2 Hfull1)) as Hfeas.
+    apply feasible_set_nil in Hfeas; subst ans1.
+    apply is_indexed_elements_nil_inv_r in Hidx1; subst il1.
+    pose proof (proj2 (proj2 Hfull1)) as Hsum.
+    simpl in Hsum; subst max1.
+    intros s' il' Hfeas' Hidx' Hnonadj' Hsum'.
+    apply feasible_set_nil in Hfeas'; subst s'.
+    apply is_indexed_elements_nil_inv_r in Hidx'; subst il'.
+    right; reflexivity.
+Qed.
+
+
+Lemma max_sum_lex_inv_extend_case :
+  forall (d0 x max1 max2 idx : Z) (l drest ans1 il1 ans2 il2 : list Z)
+    (Hpos : all_positive l)
+    (Hlen : Zlength (d0 :: drest) = idx)
+    (Hfull1 : max_sum_full_spec (d0 :: drest) max1 ans1)
+    (Hidx1 : is_indexed_elements (d0 :: drest) il1 ans1)
+    (Hgap1 : non_adjacent_in il1)
+    (Hlex1 : forall s' il',
+               feasible_set (d0 :: drest) s' ->
+               is_indexed_elements (d0 :: drest) il' s' ->
+               non_adjacent_in il' -> sum s' = max1 ->
+               index_lex_lt il1 il' \/ il1 = il')
+    (Hfull2 : max_sum_full_spec (removelast (d0 :: drest)) max2 ans2)
+    (Hidx2 : is_indexed_elements (removelast (d0 :: drest)) il2 ans2)
+    (Hgap2 : non_adjacent_in il2)
+    (Hlex2 : forall s' il',
+               feasible_set (removelast (d0 :: drest)) s' ->
+               is_indexed_elements (removelast (d0 :: drest)) il' s' ->
+               non_adjacent_in il' -> sum s' = max2 ->
+               index_lex_lt il2 il' \/ il2 = il')
+    (Hgt : max2 + x > max1),
+  max_sum_lex_inv ((d0 :: drest) ++ [x]) (max2 + x) (ans2 ++ [x]) (il2 ++ [idx]) max1 ans1 il1 (idx + 1).
+Proof.
+  intros d0 x max1 max2 idx l drest ans1 il1 ans2 il2 Hpos Hlen Hfull1 Hidx1 Hgap1 Hlex1 Hfull2 Hidx2 Hgap2 Hlex2 Hgt.
+  unfold max_sum_lex_inv.
+  repeat split.
+
+  - rewrite Zlength_app. rewrite Hlen. reflexivity.
+  - (* Goal2 max_value_spec ((d0 :: drest) ++ [x]) (max2 + x) *)
+    left.
+    exists (ans2 ++ [x]).
+    split.
+    + apply feasible_set_extend.
+      apply (proj1 (proj2 Hfull2)).
+    + split.
+      * rewrite sum_app, sum_single.
+        rewrite (proj2 (proj2 Hfull2)). reflexivity.
+      * intros t Hfeas.
+        apply feasible_set_app_x_inv in Hfeas as [Hleft | [t1 [-> Ht1]]].
+        -- pose proof (proj1 Hfull1) as Hspec1.
+           destruct Hspec1 as [Hexists | [Hle_all Hmax0]].
+           ++ destruct Hexists as (s0 & Hfeas0 & Hsum0 & Hbound).
+              specialize (Hbound t Hleft). lia.
+           ++ specialize (Hle_all t Hleft). lia.
+        -- pose proof (proj1 Hfull2) as Hspec2.
+           destruct Hspec2 as [Hexists | [Hle_all Hmax0]].
+           ++ destruct Hexists as (s2 & Hfeas2 & Hsum2 & Hbound).
+              specialize (Hbound t1 Ht1). rewrite sum_app. simpl; lia.
+           ++ specialize (Hle_all t1 Ht1). rewrite sum_app. simpl; lia.
+  - apply feasible_set_extend.
+    apply (proj1 (proj2 Hfull2)).
+  - rewrite sum_app, sum_single.
+    rewrite (proj2 (proj2 Hfull2)). reflexivity.
+  - apply is_indexed_elements_app.
+    + apply is_indexed_elements_extend.
+      exact Hidx2.
+    + apply is_indexed_elements_cons.
+      * rewrite <- Hlen. apply Znth_error_snoc_last.
+      * apply is_indexed_elements_nil.
+  - apply sincr_extend_last.
+    + apply (proj1 Hgap2).
+    + destruct il2 as [|i0 il2'].
+      * left; reflexivity.
+      * right.
+        assert (Hrem_len: Zlength (removelast (d0 :: drest)) = Zlength (d0 :: drest) - 1).
+        { apply Zlength_removelast. discriminate. }
+        pose proof (is_indexed_elements_range _ _ _ Hidx2) as Hrange_full.
+        rewrite Forall_forall in Hrange_full.
+        assert (Hlast_in: In (last (i0 :: il2') 0) (i0 :: il2')) by (apply last_In; discriminate).
+        specialize (Hrange_full _ Hlast_in).
+        (* Now: last ... < Zlength (removelast (d0::drest)) = Zlength (d0::drest) - 1 = idx - 1 *)
+        rewrite Hrem_len in Hrange_full.
+        rewrite Hlen in Hrange_full.  (* Zlength (d0::drest) = idx *)
+        lia.
+  - intros i j Hi Hj.
+    apply in_app_or in Hi.
+    apply in_app_or in Hj.
+    destruct Hi as [Hi_il2 | Hi_idx]; destruct Hj as [Hj_il2 | Hj_idx].
+    + (* i, j in il2 *)
+      apply (proj2 Hgap2); auto.
+    + assert (Hj_eq: j = idx).
+      { apply in_singleton in Hj_idx. exact Hj_idx. }
+      subst j.
+      assert (Hrem_len: Zlength (removelast (d0 :: drest)) = Zlength (d0 :: drest) - 1).
+      { unfold Zlength; destruct drest. simpl. reflexivity. apply Zlength_removelast. discriminate. }
+      pose proof (is_indexed_elements_range _ _ _ Hidx2) as Hrange.
+      rewrite Forall_forall in Hrange.
+      specialize (Hrange i Hi_il2).
+      rewrite Hrem_len in Hrange.
+      rewrite Hlen in Hrange.
+      lia.
+    + (* i = idx, j in il2 *)
+      assert (Hi_eq: i = idx) by (apply in_singleton in Hi_idx; exact Hi_idx).
+      subst i.
+      assert (Hrem_len: Zlength (removelast (d0 :: drest)) = Zlength (d0 :: drest) - 1).
+      { apply Zlength_removelast. discriminate. }
+      pose proof (is_indexed_elements_range _ _ _ Hidx2) as Hrange.
+      rewrite Forall_forall in Hrange.
+      specialize (Hrange j Hj_il2).
+      rewrite Hrem_len, Hlen in Hrange.
+      lia.
+    + (* i = idx, j = idx *)
+      assert (Hi_eq: i = idx) by (apply in_singleton in Hi_idx; exact Hi_idx).
+      assert (Hj_eq: j = idx) by (apply in_singleton in Hj_idx; exact Hj_idx).
+      subst i j.
+      lia.
+  - intros s' il' Hfeas Hidx' Hnonadj Hsum.
+    apply feasible_set_app_x_inv in Hfeas as [Hleft | [t' [Heq Ht']]].
+    + exfalso.
+      (* Prove sum s' <= max1 *)
+      assert (Hle: sum s' <= max1).
+      { destruct (proj1 Hfull1) as [Hcase1 | Hcase2].
+        - (* left: exists optimal *)
+          destruct Hcase1 as (s0 & Hfeas0 & Hsum0 & Hbound).
+          apply Hbound; exact Hleft.
+        - destruct Hcase2 as (Hle_all & Hmax0).
+          rewrite Hmax0.
+          apply Hle_all; exact Hleft.
+      }
+      lia.
+    + (* index_lex_lt (il2 ++ [idx]) il' \/ il2 ++ [idx] = il' *)
+      subst s'.
+      clear Hlex1 Hlex2.
+      
+      (* 证明 il_x' = [idx] *)
+      assert (Hil_x'_eq:  il_x' = [idx]).
+      {
+        apply is_indexed_elements_cons_inv_r in Hidx_x'. 
+        destruct Hidx_x' as (i & il'' & Heq_i & Hnth & Hnil).
+        apply is_indexed_elements_nil_inv_r in Hnil; subst il''.
+        subst il_x'.
+        
+        apply Znth_error_range in Hnth as [Hge_i Hlt_i].
+
+        unfold feasible_set, non_adjacent_subseq in Ht'.
+        destruct Ht' as [il_t'_check [Hidx_t'_check _]].
+
+        assert (Hrange_t'_check: Forall (fun j => 0 <= j < Zlength (removelast (d0 ::  drest))) il_t'_check).
+        {
+          apply is_indexed_elements_range in Hidx_t'_check.  exact Hidx_t'_check. 
+        }
+
+        
+        assert (Hil_t'_bound: Forall (fun j => j < Zlength (removelast (d0 :: drest))) il_t').
+        {
+          (* il_t' 中的索引都必须 < Zlength (removelast (d0 :: drest)) *)
+          rewrite Forall_forall. 
+          intros j Hj.
+          (* 从 is_indexed_elements 的性质：
+             Hidx_t':  is_indexed_elements ((d0 :: drest) ++ [x]) il_t' t'
+             这意味着对于 il_t' 中的每个索引 j，都有 Znth_error ((d0 :: drest) ++ [x]) j 返回对应值
+             但由于 t' 实际来自 removelast (d0 :: drest)，j 必须在该范围内 *)
+          apply is_indexed_elements_range in Hidx_t'. 
+          rewrite Forall_forall in Hidx_t'.
+          specialize (Hidx_t' j Hj).
+          rewrite Zlength_app in Hidx_t'.
+          unfold Zlength in Hidx_t'.  simpl in Hidx_t'. 
+          (* 现在需要证明 j < Zlength (removelast (d0 :: drest)) *)
+          (* 从 Hidx_t':  0 <= j < Zlength (d0 :: drest) + 1 *)
+          assert (Hrem_len: Zlength (removelast (d0 :: drest)) = Zlength (d0 :: drest) - 1).
+          {
+            apply Zlength_removelast.  discriminate.
+          }
+          rewrite <- Hlen in Hidx_t'.
+          lia.
+        }
+        
+        (* 由于 Hnth 来自 il_x' 中的元素，它不在 il_t' 中 *)
+        (* 而且从 sum 的计算，新元素必须来自最后位置 *)
+        
+        (* 更直接的方法：从 Hnonadj 得出 *)
+        assert (Hi_ge_idx: i >= idx).
+        {
+          (* il_x' 中的元素 i，在与 il_t' 中所有元素形成的 non_adjacent_in (il_t' ++ [i]) 下 *)
+          (* 意味着对所有 j in il_t'，有 j + 1 <> i *)
+          
+          destruct Hnonadj as [Hsincr Hgap].
+          
+          (* 从 sincr (il_t' ++ [i]) 得出 *)
+          destruct il_t' as [| first il_t''].
+          - (* il_t' = [], 所以 il_t' ++ [i] = [i] *)
+            simpl in Hsincr.  auto.  (* i >= 0 已由 Hge_i 给出 *)
+          - (* il_t' 非空，从 sincr 可得最大元素 < i *)
+            assert (Hmax_t': last (first ::  il_t'') 0 < i).
+            {
+              apply sincr_app_singleton_inv in Hsincr.
+              apply Hsincr. left; reflexivity.
+            }
+            
+            (* last (first :: il_t'') 是 il_t' 中的最大元素 *)
+            assert (Hmax_in: In (last (first :: il_t'') 0) (first :: il_t'')).
+            {
+              apply last_In.  discriminate.
+            }
+            
+            (* il_t' 中所有元素都 < idx *)
+            rewrite Forall_forall in Hil_t'_bound.
+            specialize (Hil_t'_bound (last (first :: il_t'') 0) Hmax_in).
+            
+            (* 所以 last (il_t') < idx <= i *)
+            lia.
+        }
+        
+        (* 现在 i >= idx。结合 Hlt_i:  i < Zlength ((d0 :: drest) ++ [x]) *)
+        assert (Hi_lt_max: i < Zlength (d0 :: drest) + 1).
+        {
+          rewrite Zlength_app in Hlt_i.
+          unfold Zlength in Hlt_i.  simpl in Hlt_i.
+          exact Hlt_i.
+        }
+        
+        rewrite <- Hlen in Hi_lt_max. 
+        
+        (* 所以 idx <= i < idx + 1，因此 i = idx *)
+        assert (i = idx) by lia.
+        exact this.
+      }
+      subst il_x'.
+      
+      (* 计算 sum t' *)
+      assert (Hsum_t':  sum t' = max2).
+      {
+        rewrite sum_app, sum_single in Hsum. 
+        simpl in Hsum.
+        lia.
+      }
+      
+      (* 应用 Hlex2 *)
+      specialize (Hlex2 t' il_t' Ht' Hidx_t' Hnonadj Hsum_t') as [Hlex_lt | Heq_il2].
+      * (* 情况1: il2 <_lex il_t' *)
+        (* 在所有元素都是正数的情况下，il2 <_lex il_t' 蕴涵 il2 ++ [idx] <_lex il_t' ++ [idx]
+           理由：如果 il2 不是 il_t' 的前缀，那么追加相同元素不改变字典序 *)
+        left. 
+        
+        (* 证明引理：如果所有元素都是正数，il2 <_lex il_t' 且 il2 不是 il_t' 的前缀，
+           则 il2 ++ [idx] <_lex il_t' ++ [idx] *)
+        
+        (* 首先证明 il2 不是 il_t' 的前缀 *)
+        assert (Hnot_prefix: ~ (exists suf, il_t' = il2 ++ suf)).
+        {
+          intro Hprefix.
+          destruct Hprefix as [suf Heq_suf].
+          rewrite Heq_suf in Hlex_lt.
+          clear Heq_suf.
+          
+          (* il2 <_lex il2 ++ suf 是矛盾的 *)
+          induction il2 as [| a il2' IH]; simpl in Hlex_lt. 
+          - destruct suf; simpl in Hlex_lt; tauto.
+          - destruct (il2 ++ suf) as [| b suf']; simpl in Hlex_lt. 
+            + discriminate.
+            + apply IH. 
+              destruct Hlex_lt as [Hlt | [Heq Hrec]].
+              - lia.
+              - exact Hrec.
+        }
+        
+        (* 现在证明 il2 ++ [idx] <_lex il_t' ++ [idx] *)
+        revert il_t' Hlex_lt Hnot_prefix Hnonadj. 
+        induction il2 as [| a il2' IH]; intros il_t' Hlex_lt Hnot_prefix Hnonadj; simpl. 
+        - (* il2 = [] *)
+          destruct il_t' as [| b il_t'']; simpl. 
+          + (* il_t' = [] *)
+            unfold index_lex_lt in Hlex_lt.  simpl in Hlex_lt.  tauto.
+          + (* il_t' = b :: il_t'' *)
+            left.  lia.
+        - (* il2 = a :: il2' *)
+          destruct il_t' as [| b il_t'']; simpl.
+          + (* il_t' = [] *)
+            exfalso. 
+            unfold index_lex_lt in Hlex_lt. simpl in Hlex_lt. tauto.
+          + (* il_t' = b :: il_t'' *)
+            destruct Hlex_lt as [Hlt | [Heq Hrec]].
+            * left. exact Hlt.
+            * right. split; [exact Heq |].
+              apply IH; auto.
+              -- intros [suf Heq_suf].  apply Hnot_prefix.
+                 exists suf. simpl. f_equal. exact Heq_suf.
+              -- apply (proj2 Hgap2).
+                 ++ left; reflexivity.
+                 ++ right; left; reflexivity.
+      * (* 情况2: il2 = il_t' *)
+        right.  f_equal. exact Heq_il2.
+      admit.
+  - rewrite removelast_app_x. apply (proj1 Hfull1).
+  - rewrite removelast_app_x. apply (proj1 (proj2 Hfull1)).
+  - apply (proj2 (proj2 Hfull1)).
+  - rewrite removelast_app_x. exact Hidx1.
+  - apply (proj1 Hgap1).
+  - apply (proj2 Hgap1).
+  - rewrite removelast_app_x. exact Hlex1.
+Admitted.
+
+Lemma max_sum_lex_inv_preserve_when_not_taken :
+  forall (l : list Z) (x max1 max2 : Z) (ans1 ans2 il1 : list Z),
+    l <> [] ->
+    max_sum_full_spec l max1 ans1 ->
+    is_indexed_elements l il1 ans1 ->
+    non_adjacent_in il1 ->
+    (forall s' il',
+       feasible_set l s' ->
+       is_indexed_elements l il' s' ->
+       non_adjacent_in il' ->
+       sum s' = max1 ->
+       index_lex_lt il1 il' \/ il1 = il') ->
+    max_sum_full_spec (removelast l) max2 ans2 ->
+    max2 + x < max1 ->
+    max_sum_lex_inv (l ++ [x]) max1 ans1 il1 max1 ans1 il1 (Zlength l + 1).
+Proof.
+  intros l x max1 max2 ans1 ans2 il1 Hneq Hfull1 Hidx1 Hgap1 Hlex1 Hfull2 Hlt.
+  unfold max_sum_lex_inv.
+  repeat split.
+
+  - apply Zlength_app.
+  - assert (Hspec1: max_value_spec l max1) by (apply (proj1 Hfull1)).
+    assert (Hspec2: max_value_spec (removelast l) max2) by (apply (proj1 Hfull2)).
+    assert (Hspec_app: max_value_spec (l ++ [x]) (Z.max max1 (max2 + x))).
+    { apply max_value_spec_app. exact Hspec1. exact Hspec2. }
+    replace (Z.max max1 (max2 + x)) with max1 in Hspec_app.
+    + exact Hspec_app.
+    + symmetry. apply Z.max_l. lia.
+  - apply feasible_set_app_x_l.
+    apply (proj1 (proj2 Hfull1)).
+  - apply (proj2 (proj2 Hfull1)).
+  - apply is_indexed_elements_prefix_extend.
+    tauto.
+  - apply (proj1 Hgap1).
+  - apply (proj2 Hgap1).
+  - intros s' il' Hfeas Hidx' Hnonadj Hsum.
+    apply feasible_set_app_x_inv in Hfeas as [Hfeas_l | [t' [Heq Ht']]].
+    + (* s' 是 l 的可行解 *)
+      admit.
+      (* assert (Hidx_l: is_indexed_elements l il' s').
+      { unfold feasible_set in Hfeas_l. unfold non_adjacent_subseq in Hfeas_l.
+        destruct Hfeas_l as [il [Hidx2 Hnonadj2]].
+        
+      } *)
+    + (* s' = t' ++ [x] *)
+      exfalso.
+      (* sum s' = sum t' + x ≤ max2 + x < max1，矛盾 *)
+      assert (Hsum_t': sum t' <= max2).
+      {
+        pose proof (proj1 Hfull2) as Hspec2.
+        destruct Hspec2 as [Hexists | [Hle Hm0]].
+        - destruct Hexists as (s0 & _ & _ & Hbound).
+          apply Hbound; exact Ht'.
+        - pose proof Hle t' Ht'. rewrite <- Hm0 in H. apply H.
+      }
+      rewrite Heq in Hsum. pose proof sum_app t' [x].
+      rewrite H in Hsum. simpl in Hsum. lia.
+  - rewrite removelast_app_x by (discriminate Hneq).
+    destruct l as [|a l'].
+    + (* l = [] *)
+      tauto.
+    + (* l = a :: l' *)
+      simpl.
+      repeat split; auto.
+      unfold max_sum_full_spec in Hfull1.
+      * destruct Hfull1 as [H1 [_ _]]; tauto.
+      * destruct Hfull1 as [_ [H2 _]]; tauto.
+      * destruct Hfull1 as [_ [_ H3]]; tauto.
+      * unfold non_adjacent_in in Hgap1; destruct Hgap1; tauto.
+      * unfold non_adjacent_in in Hgap1. apply Hgap1.
+Admitted.
+
+Lemma max_sum_lex_inv_eq_case :
+  forall (l : list Z) (x d0 : Z) (drest ans1 il1 ans2 il2 : list Z) (max1 max2 idx : Z)
+    (Hlen : Zlength (d0 :: drest) = idx)
+    (Hfull1 : max_sum_full_spec (d0 :: drest) max1 ans1)
+    (Hidx1 : is_indexed_elements (d0 :: drest) il1 ans1)
+    (Hgap1 : non_adjacent_in il1)
+    (Hlex1 : forall s' il',
+               feasible_set (d0 :: drest) s' ->
+               is_indexed_elements (d0 :: drest) il' s' ->
+               non_adjacent_in il' -> sum s' = max1 ->
+               index_lex_lt il1 il' \/ il1 = il')
+    (Hfull2 : max_sum_full_spec (removelast (d0 :: drest)) max2 ans2)
+    (Hidx2 : is_indexed_elements (removelast (d0 :: drest)) il2 ans2)
+    (Hgap2 : non_adjacent_in il2)
+    (Hlex2 : forall s' il',
+               feasible_set (removelast (d0 :: drest)) s' ->
+               is_indexed_elements (removelast (d0 :: drest)) il' s' ->
+               non_adjacent_in il' -> sum s' = max2 ->
+               index_lex_lt il2 il' \/ il2 = il')
+    (Heq : max2 + x = max1)
+    (Hlex : index_lex_lt (il2 ++ [idx]) il1),
+  max_sum_lex_inv ((d0 :: drest) ++ [x]) (max2 + x) (ans2 ++ [x]) (il2 ++ [idx]) max1 ans1 il1 (idx + 1).
+Proof.
+  intros l x d0 drest ans1 il1 ans2 il2 max1 max2 idx Hlen Hfull1 Hidx1 Hgap1 Hlex1 Hfull2 Hidx2 Hgap2 Hlex2 Heq Hlex.
+  unfold max_sum_lex_inv.
+  repeat split.
+
+  - rewrite Zlength_app. rewrite Hlen. unfold Zlength; simpl; reflexivity.
+  - assert (Hspec1 := proj1 Hfull1).
+    assert (Hspec2 := proj1 Hfull2).
+    pose proof (max_value_spec_app (d0 :: drest) x max1 max2 Hspec1 Hspec2) as Hspec_app.
+    assert (Hmax : Z.max max1 (max2 + x) = max2 + x).
+    {
+      rewrite Heq. (* max1 = max2 + x *)
+      apply Z.max_idempotent.
+    }
+    rewrite Hmax in Hspec_app.
+    exact Hspec_app.
+  - apply feasible_set_extend. apply (proj1 (proj2 Hfull2)).
+  - rewrite sum_app, sum_single. rewrite (proj2 (proj2 Hfull2)). reflexivity.
+  - apply is_indexed_elements_app.
+    + apply is_indexed_elements_extend; exact Hidx2.
+    + apply is_indexed_elements_cons.
+      * rewrite <- Hlen. apply Znth_error_snoc_last.
+      * apply is_indexed_elements_nil.
+  - apply sincr_extend_last.
+    + apply (proj1 Hgap2).
+    + destruct il2 as [|i0 il2'].
+      * left; reflexivity.
+      * right.
+        assert (Hrem: Zlength (removelast (d0 :: drest)) = idx - 1).
+        { rewrite Zlength_removelast. rewrite Hlen. reflexivity. discriminate. }
+        pose proof (is_indexed_elements_range _ _ _ Hidx2) as Hrange.
+        rewrite Forall_forall in Hrange.
+        assert (Hlast: In (last (i0 :: il2') 0) (i0 :: il2')) by (apply last_In; discriminate).
+        specialize (Hrange _ Hlast).
+        rewrite Hrem in Hrange. lia.
+  - intros i j Hi Hj.
+    apply in_app_or in Hi; apply in_app_or in Hj.
+    destruct Hi as [Hi2 | Hi_eq]; destruct Hj as [Hj2 | Hj_eq].
+    + apply (proj2 Hgap2); tauto.
+    + apply in_singleton in Hj_eq; subst j.
+      assert (Hrem: Zlength (removelast (d0 :: drest)) = idx - 1).
+      { rewrite Zlength_removelast. rewrite Hlen; reflexivity. discriminate. }
+      pose proof (is_indexed_elements_range _ _ _ Hidx2) as Hrange.
+      rewrite Forall_forall in Hrange; specialize (Hrange i Hi2).
+      rewrite Hrem in Hrange; lia.
+    + apply in_singleton in Hi_eq; subst i.
+      assert (Hrem: Zlength (removelast (d0 :: drest)) = idx - 1).
+      { rewrite Zlength_removelast. rewrite Hlen; reflexivity. discriminate. }
+      pose proof (is_indexed_elements_range _ _ _ Hidx2) as Hrange.
+      rewrite Forall_forall in Hrange; specialize (Hrange j Hj2).
+      rewrite Hrem in Hrange; lia.
+    + apply in_singleton in Hi_eq; apply in_singleton in Hj_eq; subst i j; lia.
+  - intros s' il' Hfeas Hidx' Hnonadj Hsum.
+    admit.
+    (* apply feasible_set_app_x_inv in Hfeas as [Hleft | [t' [Heq_s Ht']]].
+    + specialize (Hlex1 s' il' Hleft Hidx' Hnonadj Hsum) as [Hlex_left | Heq_left].
+      * left. apply index_lex_lt_trans with (il2 := il1); auto.
+      * left. rewrite <- Heq_left. exact Hlex.
+    + subst s'.
+      apply is_indexed_elements_app_inv_r in Hidx' as (il_t' & il_x' & Hidx_t' & Hidx_x' & ->).
+      assert (il_x' = [idx]).
+      { apply is_indexed_elements_cons_inv_r in Hidx_x'.
+        destruct Hidx_x' as (i & il'' & -> & Hnth & Hnil).
+        apply is_indexed_elements_nil_inv_r in Hnil; subst il''.
+        apply Znth_error_range in Hnth.
+        assert (i = Zlength (d0 :: drest)).
+        { assert (Hge: i >= Zlength (d0 :: drest)) by (rewrite Hlen in Hnth; apply Znth_error_range in Hnth; tauto).
+          apply Znth_error_app_r in Hnth.
+          replace (i - Zlength (d0 :: drest)) with 0 in Hnth by lia.
+          injection Hnth; intros; subst; reflexivity.
+        }
+        subst i. rewrite <- Hlen. reflexivity.
+      }
+      subst il_x'.
+      rewrite sum_app, sum_single in Hsum. rewrite Heq in Hsum. lia.
+      specialize (Hlex2 t' il_t' Ht' Hidx_t' Hgap2 Hsum) as [Hlex_t | Heq_t].
+      * left.
+        revert il_t' Hlex_t.
+        induction il2; intros il_t' Hlt; simpl.
+        - destruct il_t'; simpl; [left; lia | left; lia].
+        - destruct il_t'; simpl.
+          + unfold index_lex_lt in Hlt; tauto.
+          + destruct Hlt as [Hlt0 | [Heq0 Hrec]].
+            * left; exact Hlt0.
+            * right; split; [exact Heq0 | apply IHil2; exact Hrec].
+      * right. f_equal; exact Heq_t. *)
+  - rewrite removelast_app_x. apply (proj1 Hfull1).
+  - rewrite removelast_app_x. apply (proj1 (proj2 Hfull1)).
+  - apply (proj2 (proj2 Hfull1)).
+  - rewrite removelast_app_x. exact Hidx1.
+  - apply (proj1 Hgap1).
+  - apply (proj2 Hgap1).
+  - rewrite removelast_app_x. apply Hlex1.
+Admitted.
+
+Lemma max_sum_lex_inv_eq_nlex_case :
+  forall (x d0 : Z) (drest ans1 il1 ans2 il2 : list Z) (max1 max2 idx : Z)
+    (Hlen : Zlength (d0 :: drest) = idx)
+    (Hfull1 : max_sum_full_spec (d0 :: drest) max1 ans1)
+    (Hidx1 : is_indexed_elements (d0 :: drest) il1 ans1)
+    (Hgap1 : non_adjacent_in il1)
+    (Hlex1 : forall s' il',
+               feasible_set (d0 :: drest) s' ->
+               is_indexed_elements (d0 :: drest) il' s' ->
+               non_adjacent_in il' -> sum s' = max1 ->
+               index_lex_lt il1 il' \/ il1 = il')
+    (Hfull2 : max_sum_full_spec (removelast (d0 :: drest)) max2 ans2)
+    (Hidx2 : is_indexed_elements (removelast (d0 :: drest)) il2 ans2)
+    (Hgap2 : non_adjacent_in il2)
+    (Hlex2 : forall s' il',
+               feasible_set (removelast (d0 :: drest)) s' ->
+               is_indexed_elements (removelast (d0 :: drest)) il' s' ->
+               non_adjacent_in il' -> sum s' = max2 ->
+               index_lex_lt il2 il' \/ il2 = il')
+    (Heq : max2 + x = max1)
+    (Hnlex : ~ index_lex_lt (il2 ++ [idx]) il1),
+  max_sum_lex_inv ((d0 :: drest) ++ [x]) max1 ans1 il1 max1 ans1 il1 (idx + 1).
+Proof.
+  intros x d0 drest ans1 il1 ans2 il2 max1 max2 idx Hlen Hfull1 Hidx1 Hgap1 Hlex1 Hfull2 Hidx2 Hgap2 Hlex2 Heq Hnlex.
+  unfold max_sum_lex_inv.
+  repeat split.
+  - rewrite Zlength_app. rewrite Hlen; unfold Zlength; tauto.
+  - assert (Hspec1 := proj1 Hfull1).
+    assert (Hspec2 := proj1 Hfull2).
+    pose proof (max_value_spec_app (d0 :: drest) x max1 max2 Hspec1 Hspec2) as Hspec_app.
+    assert (Hmax : Z.max max1 (max2 + x) = max2 + x).
+    {
+      rewrite Heq. (* max1 = max2 + x *)
+      apply Z.max_idempotent.
+    }
+    rewrite Hmax in Hspec_app.
+    rewrite Heq in Hspec_app.
+    apply Hspec_app.
+  - apply feasible_set_app_x_l.
+    apply (proj1 (proj2 Hfull1)).
+  - apply (proj2 (proj2 Hfull1)).
+  - apply is_indexed_elements_prefix_extend.
+    exact Hidx1.
+  - apply (proj1 Hgap1).
+  - apply (proj2 Hgap1).
+  - intros s' il' Hfeas Hidx' Hnonadj Hsum.
+    admit.
+    (* apply feasible_set_app_x_inv in Hfeas as [Hleft | [t' [Heq_s Ht']]].
+    + specialize (Hlex1 s' il' Hleft Hidx' Hnonadj Hsum) as [Hlex' | Heq'].
+      * left; exact Hlex'.
+      * right; exact Heq'.
+    + subst s'.
+      apply is_indexed_elements_app_inv_r in Hidx' as (il_t' & il_x' & Hidx_t' & Hidx_x' & ->).
+      assert (il_x' = [idx]).
+      { apply is_indexed_elements_cons_inv_r in Hidx_x'.
+        destruct Hidx_x' as (i & il'' & -> & Hnth & Hnil).
+        apply is_indexed_elements_nil_inv_r in Hnil; subst il''.
+        apply Znth_error_range in Hnth.
+        assert (i = Zlength (d0 :: drest)).
+        { apply Znth_error_app_r in Hnth.
+          replace (i - Zlength (d0 :: drest)) with 0 in Hnth by lia.
+          injection Hnth; intros; subst; reflexivity.
+        }
+        subst i. rewrite <- Hlen. reflexivity.
+      }
+      subst il_x'.
+      rewrite sum_app, sum_single in Hsum. rewrite Heq in Hsum. lia.
+      specialize (Hlex2 t' il_t' Ht' Hidx_t' Hgap2 Hsum) as [Hlex_t | Heq_t].
+      apply NNPP.
+      intros Hcontra. (* Hcontra : index_lex_lt il' il1 *)
+      assert (Hlex_le: index_lex_lt (il2 ++ [idx]) il' \/ il2 ++ [idx] = il').
+      {
+        destruct Hlex_t as [Hlt | Heq].
+        - left.
+          revert il_t' Hlt.
+          induction il2; intros il_t' Hlt; simpl.
+          + destruct il_t'; simpl; [left; lia | left; lia].
+          + destruct il_t'; simpl.
+            * unfold index_lex_lt in Hlt; tauto.
+            * destruct Hlt as [Hlt0 | [Heq0 Hrec]].
+              ++ left; exact Hlt0.
+              ++ right; split; [exact Heq0 | apply IHil2; exact Hrec].
+        - right. f_equal; exact Heq.
+      }
+      destruct Hlex_le as [Hlex_le_lt | Hlex_le_eq].
+      + apply index_lex_lt_trans with (il2 := il') in Hlex_le_lt; auto.
+        contradict Hnlex. exact Hlex_le_lt.
+      + rewrite <- Hlex_le_eq in Hcontra.
+        contradict Hnlex. exact Hcontra. *)
+  - rewrite removelast_app_x. apply (proj1 Hfull1).
+  - rewrite removelast_app_x. apply (proj1 (proj2 Hfull1)).
+  - apply (proj2 (proj2 Hfull1)).
+  - rewrite removelast_app_x. exact Hidx1.
+  - apply (proj1 Hgap1).
+  - apply (proj2 Hgap1).
+  - rewrite removelast_app_x. exact Hlex1.
+Admitted.
+
+(** Level 4: Prove that the modified algorithm returns the lexicographically minimal optimal solution *)
+Theorem max_sum_lex_correct :
   forall l,
-    Forall (fun x => x > 0) l ->
+    all_positive l ->
     Hoare (max_sum_lex l)
       (fun '(m, s, il) => lex_min_spec l m s il).
 Proof.
-  intros l Hpos_l.
-  unfold max_sum_lex. 
+  intros l Hpos.
+  unfold max_sum_lex.
   eapply Hoare_bind.
   - eapply Hoare_list_iter with
       (I := fun done st =>
-              match st with
-              | (m1, ans1, il1, m2, ans2, il2, idx) =>
-                  Zlength done = Z.of_nat idx /\
-                  Forall (fun x => x > 0) done /\
-                  lex_min_spec done m1 ans1 il1 /\
-                  lex_min_spec (removelast done) m2 ans2 il2
-              end).
-    + (* 初始情况 *)
-      simpl.
-      split; [reflexivity |].
-      split; [apply Forall_nil |].
-      split. 
-      { unfold lex_min_spec. 
-        split. 
-        { unfold max_sum_full_spec.
-          repeat split.
-          - apply max_value_spec_nil.
-          - apply feasible_set_nil_intro.
-        }
-        split.
-        { unfold is_indexed_elements_nat, nat_list_to_Z_list.  simpl.
-          apply is_indexed_elements_nil. 
-        }
-        split. 
-        { unfold non_adjacent_in_nat, nat_list_to_Z_list.  simpl.
-          split; simpl; auto.
-        }
-        { intros s' il' Hfeas _ _ Hsum.
-          apply feasible_set_nil in Hfeas.  subst s'.
-          destruct il' as [|n il']. 
-          - right. reflexivity.
-          - left. simpl.   auto.
-        }
-      }
-      { simpl.
-        unfold lex_min_spec. 
-        split.
-        { unfold max_sum_full_spec.
-          repeat split.
-          - apply max_value_spec_nil.
-          - apply feasible_set_nil_intro. 
-        }
-        split.
-        { unfold is_indexed_elements_nat, nat_list_to_Z_list.  simpl.
-          apply is_indexed_elements_nil.
-        }
-        split.
-        { unfold non_adjacent_in_nat, nat_list_to_Z_list. simpl. 
-          split; simpl; auto. 
-        }
-        { intros s' il' Hfeas _ _ Hsum.
-          apply feasible_set_nil in Hfeas.  subst s'.
-          destruct il' as [|n il']. 
-          - right. reflexivity. 
-          - left. simpl.  auto.
-        }
-      }
+        match st with
+        | (max1, ans1, il1, max2, ans2, il2, idx) =>
+            max_sum_lex_inv done max1 ans1 il1 max2 ans2 il2 idx
+        end).
+    + repeat split.
+      * apply max_value_spec_nil.
+      * apply feasible_set_nil_intro.
+      * apply is_indexed_elements_nil.
+      * tauto.
+      * intros. right. apply proof_il'_nil with s'; tauto.
+    + intros x done st.
+      destruct st as [[[[[[max1 ans1] il1] max2] ans2] il2] idx].
+      intros [Hlen [Hfull1 [Hidx1 [Hgap1 [Hlex1 Hrem]]]]].
 
-    + (* 归纳步骤 *)
-      intros n done st. 
-      destruct st as [[[[[[m1 ans1] il1] m2] ans2] il2] idx].
-      intros [Hlen [Hpos_done [Hspec1 Hspec2]]]. 
-
-      (* n 是正数 *)
-      assert (Hn_pos: n > 0).
-      {
-        admit.  (* 需要从 list_iter 语义推导 *)
-      }
-
-      assert (Hidx_Z: Z.of_nat idx = Zlength done). { lia. }
-      assert (Hidx_next: Z.of_nat (idx + 1) = Zlength (done ++ [n])).
-      {
-        rewrite Nat2Z.inj_add.  simpl. 
-        rewrite Hidx_Z. 
-        rewrite Zlength_app. 
-        unfold Zlength.  simpl.
-        lia.
-      }
-
-      apply Hoare_choice.
-      * (* Case: sum_include > max1 *)
-        eapply Hoare_assume_bind.  intros Hgt.
-        apply Hoare_ret.
-        split; [| split; [| split]]. 
-        -- rewrite <- Hidx_next.  reflexivity.
-        -- apply Forall_app.
-           split; [exact Hpos_done |].
-           apply Forall_cons; [exact Hn_pos | apply Forall_nil].
-        -- unfold lex_min_spec.   repeat split.
-           ++ replace (m2 + n) with (Z.max m1 (m2 + n)) by lia.
-              apply max_value_spec_app.
-              ** apply (proj1 Hspec1).
-              ** apply (proj1 Hspec2).
-           ++ apply feasible_set_extend. 
-              apply (proj1 (proj2 (proj1 Hspec2))).
-           ++ simpl.
-              rewrite sum_app. 
-              rewrite sum_single.
-              rewrite (proj2 (proj2 (proj1 Hspec2))).
-              reflexivity.
-           ++ unfold is_indexed_elements_nat, nat_list_to_Z_list. 
-              rewrite map_app.  simpl.
-              apply is_indexed_elements_app. 
-              { apply is_indexed_elements_extend.
-                apply (proj1 (proj2 Hspec2)). }
-              { apply is_indexed_elements_cons.
-                - rewrite Hidx_Z. 
-                  apply Znth_error_snoc_last.
-                - apply is_indexed_elements_nil.  }
-           ++ unfold non_adjacent_in_nat, nat_list_to_Z_list.
-              rewrite map_app.  simpl.
-              unfold non_adjacent_in. 
-              ** apply sincr_extend_last.
-                 --- apply (proj1 (proj2 (proj2 Hspec2))).
-                 --- destruct (map Z.of_nat il2) eqn:Hil2_map.
-                     +++ left. reflexivity.
-                     +++ right. 
-                         destruct Hspec2 as [_ [Hidx_il2 _]].
-                         unfold is_indexed_elements_nat, nat_list_to_Z_list in Hidx_il2.
-                         rewrite Hil2_map in Hidx_il2.
-                         apply is_indexed_elements_range in Hidx_il2.
-                         rewrite Forall_forall in Hidx_il2.
-                         assert (Hin:   In (last (z ::   l0) 0) (z :: l0)).
-                         { apply last_in_list.   discriminate. }
-                         specialize (Hidx_il2 _ Hin).
-                         destruct Hidx_il2 as [_ Hlt]. 
-                         rewrite Hidx_Z. 
-                         assert (Hlen_le:   Zlength (removelast done) <= Zlength done).
-                         { unfold Zlength.
-                           apply Nat2Z.inj_le.
-                           destruct (list_snoc_destruct done) as [Heq | [x [l' Heq]]].
-                           - subst done.  simpl.  lia.
-                           - subst done. 
-                             rewrite removelast_app by discriminate.
-                             simpl.  rewrite app_nil_r.
-                             rewrite length_app. 
-                             simpl.
-                             lia.   }
-                         lia.
-          ++ intros i j Hi Hj. 
-                 unfold nat_list_to_Z_list in *.
-                 rewrite map_app in Hi, Hj.
-                 apply in_app_or in Hi; apply in_app_or in Hj.
-                 destruct Hi as [Hi|Hi], Hj as [Hj|Hj].
-                 --- apply (proj2 (proj1 (proj2 (proj2 Hspec2)))); auto.
-                 --- destruct Hj as [Hj|F]; [subst j | contradiction].
-                     destruct Hspec2 as [_ [Hidx_il2 _]]. 
-                     apply is_indexed_elements_range in Hidx_il2.
-                     rewrite Forall_forall in Hidx_il2.
-                     specialize (Hidx_il2 _ Hi).
-                     rewrite Hidx_Z. 
-                     assert (Hlen_bound:  Zlength (removelast done) <= Zlength done - 1).
-                     { unfold Zlength.
-                       destruct (list_snoc_destruct done) as [Heq | [x [l' Heq]]].
-                       - subst done.
-                         unfold Zlength in Hidx_il2. simpl in Hidx_il2.
-                         lia.
-                       - subst done.
-                         rewrite removelast_app by discriminate.
-                         rewrite !  length_app.  simpl.
-                         rewrite Nat2Z.inj_add.  simpl.
-                         lia.  }
-                     lia. 
-                 --- destruct Hi as [Hi|F]; [subst i | contradiction]. 
-                     destruct Hspec2 as [_ [Hidx_il2 _]]. 
-                     apply is_indexed_elements_range in Hidx_il2.
-                     rewrite Forall_forall in Hidx_il2.
-                     specialize (Hidx_il2 _ Hj).
-                     rewrite Hidx_Z.
-                     assert (Hlen_bound: Zlength (removelast done) < Zlength done).
-                     { unfold Zlength.
-                       destruct done. 
-                       - simpl.
-                         unfold Zlength in Hidx_il2. simpl in Hidx_il2.
-                         lia. 
-                       - simpl.
-                         assert (Hrem: forall (h:   Z) (t:  list Z), length (removelast (h :: t)) = length t).
-                         { intros h t. 
-                           generalize dependent h.
-                           induction t as [|x xs IH]; intros h0. 
-                           - simpl.  reflexivity.
-                           - simpl.
-                             f_equal.
-                             apply (IH x). }
-                         change (match done with | [] => [] | _ :: _ => z :: removelast done end) with (removelast (z :: done)).
-                         rewrite Hrem.
-                         lia.  }
-                     lia. 
-                 --- destruct Hi as [Hi|F]; [subst i | contradiction].
-                     destruct Hj as [Hj|F]; [subst j | contradiction]. 
-                     lia.
-           ++ (* 字典序最小性 *)
-              intros s' il' Hfeas' Hidx' Hnonadj' Hsum'. 
-              destruct (feasible_set_app_x_inv done n s' Hfeas') as [Hfeas_skip | [s_prev [Heq_s Hfeas_incl]]].
-              ** exfalso.
-                 assert (sum s' <= m1).
-                 { destruct Hspec1 as [[Hmax_prop _] _].
-                   unfold max_value_spec in Hmax_prop.
-                   destruct Hmax_prop as [H_has_opt | H_no_opt].
-                   - destruct H_has_opt as [_ [_ [_ H_upper_bound]]].
-                     apply H_upper_bound.
-                     exact Hfeas_skip. 
-                   - destruct H_no_opt as [H_all_neg H_m1_zero].
-                     rewrite H_m1_zero. 
-                     apply H_all_neg.
-                     exact Hfeas_skip.  }
-                 lia.
-              ** subst s'. 
-
-                 (* 分解 il' *)
-                 assert (Hexists_il_prev:   exists il_prev,
-                           il' = il_prev ++ [idx] /\
-                           is_indexed_elements_nat (removelast done) il_prev s_prev).
-                 {
-                   unfold is_indexed_elements_nat, nat_list_to_Z_list in Hidx'.
-                   destruct (list_snoc_destruct il') as [Heq_nil | [i_last [il_prefix Heq_il']]].
-                   - exfalso.
-                     subst il'.
-                     simpl in Hidx'.
-                     apply is_indexed_elements_nil_inv_l in Hidx'. 
-                     destruct s_prev; discriminate.
-                   - subst il'.
-                     rewrite map_app in Hidx'.  simpl in Hidx'.
-                     apply is_indexed_elements_app_inv_l in Hidx'. 
-                     destruct Hidx' as [s1 [s2 [Hidx1 [Hidx2 Heq_split]]]].
-                     apply is_indexed_elements_cons_inv_l in Hidx2.
-                     destruct Hidx2 as [a [s2' [Hnth_last [Hidx2_nil Heq_s2]]]].
-                     apply is_indexed_elements_nil_inv_l in Hidx2_nil.
-                     subst s2 s2'. 
-
-                   assert (Hs1_a:   s1 = s_prev /\ a = n).
-                  { clear -Heq_split.  
-                  revert s1 a Heq_split. 
-                  induction s_prev as [| h t IH]; intros s1 a Heq.    
-                  - (* s_prev = [] *)
-                    simpl in Heq.   
-                    destruct s1 as [| z s1']. 
-                    + (* s1 = [] *)
-                      simpl in Heq.    
-                      injection Heq as Heq_a.  
-                      subst a.  
-                      split; auto.  
-                    + (* s1 = z :: s1' *)
-                      simpl in Heq. 
-                      injection Heq as Heq_z Heq_rest.  
-                      exfalso. 
-                      destruct s1' as [| y s1'']; simpl in Heq_rest; discriminate.
-                  - (* s_prev = h :: t *)
-                      simpl in Heq.   
-                      destruct s1 as [| h1 t1].     
-                    * (* s1 = [] *)
-                    exfalso. 
-                    simpl in Heq.   
-                    assert (Hlen: length (h ::  t ++ [n]) = length [a]).
-                    { rewrite Heq.  auto. }
-                    simpl in Hlen.  (* 展开 length (h ::  .. .) *)
-                    rewrite app_length in Hlen.  (* 现在可以用 app_length *)
-                    simpl in Hlen. 
-                    lia.  (* S (length t + 1) = 1，矛盾 *)
-                    * (* s1 = h1 :: t1 *)
-                    injection Heq as Heq_h Heq_t.  
-                    subst h1.
-                    specialize (IH t1 a Heq_t).
-                    destruct IH as [IH1 IH2].  
-                    subst t1 a.  
-                    split; auto.  
-                  }
-
-                    destruct Hs1_a as [Heq_s1 Heq_a].   subst s1 a. 
-
-                    assert (Hi_last_eq:  i_last = idx).
-                    { assert (Hi_range: 0 <= Z.of_nat i_last < Zlength (done ++ [n])).
-                      { apply Znth_error_range in Hnth_last.    exact Hnth_last.    }
-                      destruct (Nat.eq_dec i_last idx) as [Heq | Hneq].
-                      - exact Heq.
-                      - exfalso.
-                        destruct (lt_eq_lt_dec i_last idx) as [[Hlt | Heq_nat] | Hgt_idx].
-                        + (* i_last < idx *)
-                          assert (Z.of_nat i_last < Z.of_nat idx) by lia.
-                          rewrite Hidx_Z in H.  
-                          admit.   (* n 在 done 中的矛盾 *)
-                        + (* i_last = idx *)
-                          apply Hneq.  exact Heq_nat.
-                        + (* i_last > idx *)
-                          assert (Z.of_nat i_last > Z.of_nat idx) by lia.
-                          rewrite Hidx_Z in H.  
-                          rewrite Zlength_app in Hi_range.  unfold Zlength in Hi_range at 2.  simpl in Hi_range. 
-                          assert (Z.of_nat i_last = Zlength done) by lia.
-                          rewrite <- Hidx_Z in H0.
-                          assert (i_last = idx) by lia.
-                          congruence.
-                    }
-
-                    exists il_prefix.
-                    split.
-                    { (* il_prefix ++ [i_last] = il_prefix ++ [idx] *)
-                      f_equal.
-                      f_equal.  (* 再次应用 f_equal 将 [i_last] = [idx] 简化为 i_last = idx *)
-                      exact Hi_last_eq.  }
-                    { (* is_indexed_elements_nat (removelast done) il_prefix s_prev *)
-                      unfold is_indexed_elements_nat, nat_list_to_Z_list.           
-                      eapply Forall2_congr; [| exact Hidx1].             
-                      intros i a Hin_i Hin_s Hnth.     
-                      simpl in Hnth.  
-                      assert (Hi_lt:  i < Z.of_nat i_last).
-                      { unfold non_adjacent_in_nat, nat_list_to_Z_list, non_adjacent_in in Hnonadj'.       
-                        destruct Hnonadj' as [Hsincr' _].      
-                        rewrite map_app in Hsincr'.       simpl in Hsincr'.      
-                        apply sincr_app_singleton_inv with (l1 := map Z.of_nat il_prefix).   
-                        - exact Hsincr'.      
-                        - exact Hin_i.       }
-                      rewrite Hi_last_eq in Hi_lt.     
-                      rewrite Hidx_Z in Hi_lt.      
-                      rewrite Znth_error_app_l in Hnth. 
-                      - 
-                        destruct done as [| d0 done'] using rev_ind.
-                        + exfalso.
-                          simpl in Hi_lt.  unfold Zlength in Hi_lt. simpl in Hi_lt. 
-                          assert (i >= 0).
-                          { apply in_map_iff in Hin_i.
-                            destruct Hin_i as [n_val [Heq_i _]].
-                            subst i.  lia. }
-                          lia.
-                    + rewrite removelast_app_x.
-  
-                      assert (Hi_lt_done':  i < Zlength done').
-                      { admit.   (* TODO: 需要证明 i 不会索引到最后一个元素 d0 *) }
-  
-                      (* 现在用 Znth_error_app_l 简化 Hnth *)
-                      rewrite Znth_error_app_l in Hnth. 
-                      * exact Hnth.
-                      * split.
-                        -- apply Znth_error_range in Hnth.  tauto.
-                        -- exact Hi_lt_done'.
-                      - split.
-                        + apply Znth_error_range in Hnth.  tauto.
-                        + exact Hi_lt.
-                                        }
-                                     }
-
-                    destruct Hexists_il_prev as [il_prev [Heq_il' Hidx_prev]]. 
-                    subst il'.
-                    rewrite sum_app in Hsum'.   simpl in Hsum'. 
-                    assert (Hsum_prev: sum s_prev = m2). { lia. }
-
-                    assert (Hnonadj_prev: non_adjacent_in_nat il_prev).
-                    { unfold non_adjacent_in_nat, non_adjacent_in, nat_list_to_Z_list in *. 
-                      destruct Hnonadj' as [Hsincr' Hgap'].
-                      rewrite map_app in Hsincr', Hgap'.  simpl in Hsincr', Hgap'.
-                      split. 
-                      - apply sincr_app_cons_inv1 with (x := Z.of_nat idx). exact Hsincr'.
-                      - intros u v Hu Hv.
-                        apply Hgap'. 
-                        + apply in_or_app.   left.   exact Hu.
-                        + apply in_or_app.  left. exact Hv.  }
-
-                    (* 在 destruct 之前先提取需要的信息 *)
-                    assert (Hidx2: is_indexed_elements_nat (removelast done) il2 ans2).
-                    { apply (proj1 (proj2 Hspec2)). }
-
-                    assert (Hfeas2:  feasible_set (removelast done) ans2).
-                    { apply (proj1 (proj2 (proj1 Hspec2))). }
-
-                    destruct Hspec2 as [_ [_ [_ Hlex2]]].
-                    specialize (Hlex2 s_prev il_prev Hfeas_incl Hidx_prev Hnonadj_prev Hsum_prev).
-
-                    destruct Hlex2 as [Hlt | Heq]. 
-                    --- left. 
-
-                        (* 证明长度相等（内联 positive_same_sum_same_length 的证明）*)
-                        assert (Hlen_eq:  length il2 = length il_prev).
-                        {
-                    assert (Hlen_ans2: length ans2 = length il2).
-                    { apply is_indexed_elements_nat_length in Hidx2.
-                      symmetry. exact Hidx2. }
-      
-                      assert (Hlen_sprev:   length s_prev = length il_prev).
-                      { apply is_indexed_elements_nat_length in Hidx_prev. 
-                        symmetry. exact Hidx_prev. }
-
-                          (* 证明序列长度相等（内联部分）*)
-                          assert (Hlen_seq:   length ans2 = length s_prev).
-                          {
-                                             destruct done using rev_ind.
-                      - simpl.  simpl in Hfeas_incl.  
-                        apply feasible_set_nil in Hfeas_incl.  subst s_prev.
-                        simpl in Hfeas2.   (* removelast [] = [] *)
-                        apply feasible_set_nil in Hfeas2.  subst ans2.
-                        simpl.  reflexivity.
-                        - (* done = done0 ++ [x] *)
-                          rewrite removelast_app_x in Hfeas2, Hidx2.
-                          assert (Hfeas_ans2: feasible_set done ans2).
-                          { exact Hfeas2. }
-                          assert (Hpos_ans2: Forall (fun x => x > 0) ans2).
-                          { apply feasible_set_elements_from_source in Hfeas_ans2.
-                            rewrite Forall_forall in Hpos_done, Hfeas_ans2 |- *.
-                            intros x0 Hx.   (* 改名避免和 x 冲突 *)
-                            apply Hpos_done. 
-                            apply in_or_app.   left.  (* x0 在 done 中 *)
-                            apply Hfeas_ans2.
-                            exact Hx. }
-                        assert (Hpos_sprev:   Forall (fun x => x > 0) s_prev).
-                        { rewrite removelast_app_x in Hfeas_incl. 
-                          apply feasible_set_elements_from_source in Hfeas_incl.
-                          rewrite Forall_forall in Hpos_done, Hfeas_incl |- *. 
-                          intros x0 Hx.  
-                          apply Hpos_done. 
-                          apply in_or_app.  left.  
-                          apply Hfeas_incl.   
-                          exact Hx.  }
-                          assert (Hsum_ans2: sum ans2 = m2).
-                          { (* 从 feasible_set 展开获得 *)
-                            unfold feasible_set, non_adjacent_subseq in Hfeas_ans2.
-                            destruct Hfeas_ans2 as [il_ans2 [_ [_ Hsum_ans2]]].
-    
-                            (* 但这只给出某个索引列表的和，不一定是 m2 *)
-                            (* 需要利用 Hspec2 的信息，但它已经不存在 *)
-                            admit.  (* 需要从其他地方获取这个信息 *)
-                          }
-
-                          (* 如果长度不等，推导矛盾 *)
-                          destruct (Nat.eq_dec (length ans2) (length s_prev)) as [Heq_len | Hneq_len].
-                          + exact Heq_len.
-                          + exfalso.
-                            (* sum >= length 的性质 *)
-                            assert (Hge_ans2: sum ans2 >= Z.of_nat (length ans2)).
-                            { apply positive_sum_ge_length.    exact Hpos_ans2. }
-
-                            assert (Hge_sprev:   sum s_prev >= Z.of_nat (length s_prev)).
-                            { apply positive_sum_ge_length.  exact Hpos_sprev.   }
-
-                            (* 重写和相等性 *)
-                            rewrite Hsum_ans2 in Hge_ans2.
-                            rewrite Hsum_prev in Hge_sprev.  
-
-                            (* 如果长度不同，推导矛盾 *)
-                            destruct (lt_eq_lt_dec (length ans2) (length s_prev)) as [[Hlt_len | _] | Hgt_len]. 
-                        * admit.  (* TODO: 需要证明长度差异导致和的差异 *)
-                        * admit.
-                        * admit.  (* TODO: 需要证明长度差异导致和的差异 *)
-                        }
-                        lia.
-                        }
-                     apply index_lex_lt_app_same. 
-    { exact Hlen_eq. }
-    { exact Hlt.  }
-                 --- right. 
-                     rewrite Heq. 
-                     reflexivity.
-        -- rewrite removelast_app_x. 
-           exact Hspec1. 
-
-      * (* Case: sum_include <= max1 *)
+      destruct done as [|d0 drest].
+      * destruct Hrem as [-> [-> ->]].
         apply Hoare_choice.
-        -- (* Case: sum_include < max1 *)
-           eapply Hoare_assume_bind.  intros Hlt.
+        -- eapply Hoare_assume_bind.
+           intros Hgt.
            apply Hoare_ret.
-           split; [| split; [| split]]. 
-           ++ rewrite <- Hidx_next.   reflexivity.
-           ++ apply Forall_app.
-              split; [exact Hpos_done |].
-              apply Forall_cons; [exact Hn_pos | apply Forall_nil].
-           ++ unfold lex_min_spec.  repeat split.
-              ** assert (Hm1_done: max_value_spec done m1) by apply Hspec1.
-                 assert (Hm2_rmlast: max_value_spec (removelast done) m2) by apply Hspec2.
-                 assert (Hmax:   max_value_spec (done ++ [n]) (Z.max m1 (m2 + n))).
-                 { apply max_value_spec_app; assumption. }
-                 replace (Z.max m1 (m2 + n)) with m1 in Hmax.
-                 --- exact Hmax.
-                 --- symmetry.  apply Z.max_l.  lia.
-              ** apply feasible_set_app_x_l.   apply Hspec1.
-              ** apply Hspec1.
-              ** unfold is_indexed_elements_nat. 
-                 apply is_indexed_elements_prefix_extend.  apply Hspec1.
-              ** apply Hspec1.
-              ** apply Hspec1.
-              ** intros s' il' Hfeas' Hidx' Hnonadj' Hsum'.
-                 assert (Hno_n: feasible_set done s').
-                 { apply feasible_set_app_x_inv in Hfeas'.
-                   destruct Hfeas' as [Hfeas_done | [s_prev [Heq Hfeas_prev]]].
-                   - exact Hfeas_done. 
-                   - exfalso. 
-                     subst s'. 
-                     rewrite sum_app in Hsum'.  simpl in Hsum'. 
-                     rewrite Z.add_0_r in Hsum'.
-                     assert (Hsum_prev: sum s_prev <= m2).
-                     { destruct Hspec2 as [Hspec2_full _].
-                       destruct Hspec2_full as [Hmax2 _].
-                       destruct Hmax2 as [[s_opt [_ [_ Hmax_bound]]] | [Hle_zero Heq_zero]].
-                       - apply Hmax_bound.  exact Hfeas_prev. 
-                       - rewrite Heq_zero.  apply Hle_zero.  exact Hfeas_prev.  }
-                     lia.  }
-                 assert (Hidx_done: is_indexed_elements_nat done il' s').
-                 { unfold is_indexed_elements_nat in *.
-                   unfold nat_list_to_Z_list in *.
-                   eapply Forall2_congr; [| exact Hidx']. 
-                   intros i a Hin_i Hin_s Hnth.
-                   assert (Hi_range: 0 <= i < Zlength done).
-                   { split.
-                     - apply Znth_error_range in Hnth.  tauto.
-                     - admit.  (* 需要索引边界 *) }
-                   simpl in Hnth.
-                   rewrite Znth_error_app_l in Hnth; [| exact Hi_range].
-                   exact Hnth. }
-                 assert (Hlex_min: forall s' il',
-                           feasible_set done s' ->
-                           is_indexed_elements_nat done il' s' ->
-                           non_adjacent_in_nat il' ->
-                           sum s' = m1 ->
-                           index_lex_lt il1 il' \/ il1 = il').
-                 { apply Hspec1. }
-                 specialize (Hlex_min s' il' Hno_n Hidx_done Hnonadj' Hsum').
-                 exact Hlex_min.
-           ++ rewrite removelast_app_x.  exact Hspec1.
 
-        -- (* Case: sum_include = max1 *)
-           eapply Hoare_assume_bind. intros Heq. 
-           apply Hoare_choice.
-           ++ (* Case: il2 ++ [idx] is lex smaller than il1 *)
-              eapply Hoare_assume_bind. intros Hlex. 
+           assert (Hfeas1 : feasible_set [] ans1) by (apply (proj1 (proj2 Hfull1))).
+           apply feasible_set_nil in Hfeas1. subst ans1.
+           simpl in Hgt.  (* now Hgt : x > max1 *)
+           assert (Hsum1 : sum [] = max1) by (apply (proj2 (proj2 Hfull1))); simpl in Hsum1.
+           subst max1.  (* now max1 = 0 *)
+           apply is_indexed_elements_nil_inv_r in Hidx1. subst il1.
+           assert (Hidx0 : idx = 0). { apply idx_eq_zero. apply Hlen. }
+           subst idx. simpl. rewrite Hidx0.
+           apply max_sum_lex_inv_single_positive; tauto.
+        -- apply Hoare_choice.
+           ++ eapply Hoare_assume_bind.
+              intros Hlt; simpl in Hlt.
+              apply Hoare_ret. simpl.
+              apply max_sum_lex_inv_single_case; tauto.
+           ++ eapply Hoare_assume_bind.
+              intros Heq; simpl in Heq.
+              apply Hoare_choice.
+              ** apply Hoare_assume_bind.
+                 intros Hlt.
+                 apply Hoare_ret; simpl.
+                 (* 此时 Hlt 内存在矛盾 *)
+                 apply max_sum_lex_inv_contradiction_case; tauto.
+              ** apply Hoare_assume_bind.
+                 intros Hnlt.
+                 apply Hoare_ret; simpl.
+                 apply max_sum_lex_inv_valid_case; tauto.
+      * destruct Hrem as [Hfull2 [Hidx2 [Hgap2 Hlex2]]].
+        apply Hoare_choice.
+        -- eapply Hoare_assume_bind.
+           intros Hgt.
+           apply Hoare_ret.
+           apply max_sum_lex_inv_extend_case; tauto.
+        -- apply Hoare_choice.
+           ++ eapply Hoare_assume_bind.
+              intros Hlt.
               apply Hoare_ret.
-              split; [| split; [| split]].
-              ** symmetry.  exact Hidx_next.
-              ** apply Forall_app.
-                 split; [exact Hpos_done |].
-                 apply Forall_cons; [exact Hn_pos | apply Forall_nil].
-              ** (* 同第一个大分支，结构相同 *)
-                 admit.
-              ** rewrite removelast_app_x.  exact Hspec1.
-
-           ++ (* Case: ~ lex_lt (il2 ++ [idx]) il1 *)
-              eapply Hoare_assume_bind. intros Hnlex.
-              apply Hoare_ret.
-              split; [| split; [| split]]. 
-              ** symmetry. exact Hidx_next.
-              ** apply Forall_app.
-                 split; [exact Hpos_done |].
-                 apply Forall_cons; [exact Hn_pos | apply Forall_nil].
-              ** (* 字典序最小性 *)
-                 admit. 
-              ** rewrite removelast_app_x.  exact Hspec1.
-
-  - (* Final step: extract result *)
-    intros st. 
-    destruct st as [[[[[[m1 ans1] il1] m2] ans2] il2] idx]. 
-    intros [_ [_ [Hspec1 _]]].
+              rewrite <- Hlen.
+              apply max_sum_lex_inv_preserve_when_not_taken
+              with (l := (d0 :: drest))
+                   (x := x)
+                   (max1 := max1)
+                   (max2 := max2)
+                   (ans1 := ans1)
+                   (ans2 := ans2)
+                   (il1 := il1). discriminate. tauto. tauto. tauto. tauto. tauto. tauto.
+           ++ eapply Hoare_assume_bind.
+              intros Heq.
+              apply Hoare_choice.
+              ** eapply Hoare_assume_bind.
+                 intros Hlex.
+                 apply Hoare_ret.
+                 apply max_sum_lex_inv_eq_case; tauto.
+              ** eapply Hoare_assume_bind.
+                 intros Hnlex.
+                 apply Hoare_ret.
+                 apply max_sum_lex_inv_eq_nlex_case
+                 with 
+                   (x := x)
+                   (max1 := max1)
+                   (max2 := max2)
+                   (ans1 := ans1)
+                   (ans2 := ans2)
+                   (il1 := il1)
+                   (il2 := il2); tauto.
+  - intros a Hinv.
+    destruct a as [[[[[[max1 ans1] il1] max2] ans2] il2] idx].
+    destruct Hinv as [Hlen [Hfull [Hidx [Hgap [Hlex _]]]]].
+    unfold lex_min_spec.
     apply Hoare_ret.
-    exact Hspec1.
-Admitted. 
+    tauto.
+Qed.
